vale/code/arch/x64/X64.Leakage.fst
@@ -63,33 +63,33 @@ let eq_xmms (xmms1 xmms2:xmms_taint) : (b:bool{b <==> (xmms1 == xmms2)})  =
   assert (FStar.FunctionalExtensionality.feq xmms1 xmms2 <==> b);
   b
 
-let eq_taintStates (ts1 ts2:taintState) : (b:bool{b <==> ts1 == ts2}) =
+let eq_taintStates (ts1 ts2:analysis_taints) : (b:bool{b <==> ts1 == ts2}) =
     eq_registers ts1.regTaint ts2.regTaint && ts1.flagsTaint = ts2.flagsTaint && ts1.cfFlagsTaint = ts2.cfFlagsTaint && ts1.ofFlagsTaint = ts2.ofFlagsTaint && eq_xmms ts1.xmmTaint ts2.xmmTaint
 
-let taintstate_monotone (ts ts':taintState) = ( forall r. Public? (ts'.regTaint r) ==> Public? (ts.regTaint r)) /\ (Public? (ts'.flagsTaint) ==> Public? (ts.flagsTaint)) /\
+let taintstate_monotone (ts ts':analysis_taints) = ( forall r. Public? (ts'.regTaint r) ==> Public? (ts.regTaint r)) /\ (Public? (ts'.flagsTaint) ==> Public? (ts.flagsTaint)) /\
   (Public? (ts'.cfFlagsTaint) ==> Public? (ts.cfFlagsTaint)) /\
   (Public? (ts'.ofFlagsTaint) ==> Public? (ts.ofFlagsTaint)) /\
   (forall x. Public? (ts'.xmmTaint x) ==> Public? (ts.xmmTaint x))
 
-let taintstate_monotone_trans (ts1:taintState) (ts2:taintState) (ts3:taintState)
+let taintstate_monotone_trans (ts1:analysis_taints) (ts2:analysis_taints) (ts3:analysis_taints)
   :Lemma (taintstate_monotone ts1 ts2 /\ taintstate_monotone ts2 ts3 ==> taintstate_monotone ts1 ts3) = ()
 
-let isConstant_monotone (ts1:taintState) (ts2:taintState) (code:tainted_code) (fuel:nat) (s1:traceState) (s2:traceState) 
+let isConstant_monotone (ts1:analysis_taints) (ts2:analysis_taints) (code:tainted_code) (fuel:nat) (s1:S.machine_state) (s2:S.machine_state) 
   :Lemma (isConstantTimeGivenStates code fuel ts2 s1 s2 /\ taintstate_monotone ts1 ts2 ==> isConstantTimeGivenStates code fuel ts1 s1 s2)
   = ()
 
-let isExplicit_monotone (ts:taintState) (ts1:taintState) (ts2:taintState) (code:tainted_code) 
-  (fuel:nat) (s1:traceState) (s2:traceState) 
+let isExplicit_monotone (ts:analysis_taints) (ts1:analysis_taints) (ts2:analysis_taints) (code:tainted_code) 
+  (fuel:nat) (s1:S.machine_state) (s2:S.machine_state) 
   :Lemma (isExplicitLeakageFreeGivenStates code fuel ts ts1 s1 s2 /\ taintstate_monotone ts1 ts2 ==> isExplicitLeakageFreeGivenStates code fuel ts ts2 s1 s2)
   = ()
 
-let isExplicit_monotone2 (ts:taintState) (ts1:taintState) (ts2:taintState)
-  (code:tainted_code) (fuel:nat) (s1:traceState) (s2:traceState) 
+let isExplicit_monotone2 (ts:analysis_taints) (ts1:analysis_taints) (ts2:analysis_taints)
+  (code:tainted_code) (fuel:nat) (s1:S.machine_state) (s2:S.machine_state) 
   :Lemma (isExplicitLeakageFreeGivenStates code fuel ts2 ts s1 s2 /\ taintstate_monotone ts1 ts2 ==> isExplicitLeakageFreeGivenStates code fuel ts1 ts s1 s2)
   = ()
 
-let combine_taint_states (ts1:taintState) (ts2:taintState) : (ts:taintState{taintstate_monotone ts1 ts /\ taintstate_monotone ts2 ts}) =
-  TaintState (combine_reg_taints ts1.regTaint ts2.regTaint)
+let combine_taint_states (ts1:analysis_taints) (ts2:analysis_taints) : (ts:analysis_taints{taintstate_monotone ts1 ts /\ taintstate_monotone ts2 ts}) =
+  AnalysisTaints (combine_reg_taints ts1.regTaint ts2.regTaint)
     (merge_taint ts1.flagsTaint ts2.flagsTaint)
     (merge_taint ts1.cfFlagsTaint ts2.cfFlagsTaint)
     (merge_taint ts1.ofFlagsTaint ts2.ofFlagsTaint)
@@ -115,11 +115,11 @@ let count_public_registers (regs:reg_taint) : nat =
   count_public_register regs rR14 +
   count_public_register regs rR15
 
-let count_flagTaint (ts:taintState) : nat = if Public? ts.flagsTaint then 1 else 0
+let count_flagTaint (ts:analysis_taints) : nat = if Public? ts.flagsTaint then 1 else 0
 
-let count_cfFlagTaint (ts:taintState) : nat = if Public? ts.cfFlagsTaint then 1 else 0
+let count_cfFlagTaint (ts:analysis_taints) : nat = if Public? ts.cfFlagsTaint then 1 else 0
 
-let count_ofFlagTaint (ts:taintState) : nat = if Public? ts.ofFlagsTaint then 1 else 0
+let count_ofFlagTaint (ts:analysis_taints) : nat = if Public? ts.ofFlagsTaint then 1 else 0
 
 let count_public_xmm (xmms:xmms_taint) (x:xmm) : nat = if Public? (xmms x) then 1 else 0
 
@@ -141,7 +141,7 @@ let count_public_xmms (xmms:xmms_taint) : nat =
   count_public_xmm xmms 14 +
   count_public_xmm xmms 15
 
-let count_publics (ts:taintState) : nat =
+let count_publics (ts:analysis_taints) : nat =
   count_public_registers ts.regTaint +
   count_flagTaint ts +
   count_cfFlagTaint ts +
@@ -151,7 +151,7 @@ let count_publics (ts:taintState) : nat =
 #set-options "--z3rlimit 50"
 
 #push-options "--z3rlimit 100 --max_fuel 0 --max_ifuel 1 --initial_ifuel 1"
-let monotone_decreases_count (ts ts':taintState) : Lemma
+let monotone_decreases_count (ts ts':analysis_taints) : Lemma
   (requires taintstate_monotone ts ts' /\ not (eq_taintStates ts ts'))
   (ensures count_publics ts' < count_publics ts)  
   =
@@ -163,13 +163,13 @@ let monotone_decreases_count (ts ts':taintState) : Lemma
   
 #pop-options
 
-val check_if_block_consumes_fixed_time: (block:tainted_codes) -> (ts:taintState) -> Tot (bool * taintState)
+val check_if_block_consumes_fixed_time: (block:tainted_codes) -> (ts:analysis_taints) -> Tot (bool * analysis_taints)
 (decreases %[block])
-val check_if_code_consumes_fixed_time: (code:tainted_code) -> (ts:taintState) -> Tot (bool * taintState) (decreases %[code; count_publics ts; 1])
-val check_if_loop_consumes_fixed_time: (code:tainted_code{While? code}) -> (ts:taintState) -> Tot (bool * taintState) (decreases %[code; count_publics ts; 0])
+val check_if_code_consumes_fixed_time: (code:tainted_code) -> (ts:analysis_taints) -> Tot (bool * analysis_taints) (decreases %[code; count_publics ts; 1])
+val check_if_loop_consumes_fixed_time: (code:tainted_code{While? code}) -> (ts:analysis_taints) -> Tot (bool * analysis_taints) (decreases %[code; count_publics ts; 0])
 
 #set-options "--z3refresh --z3rlimit 600"
-let rec check_if_block_consumes_fixed_time (block:tainted_codes) (ts:taintState) : bool * taintState =
+let rec check_if_block_consumes_fixed_time (block:tainted_codes) (ts:analysis_taints) : bool * analysis_taints =
   match block with
   | [] -> true, ts
   | hd::tl -> let fixedTime, ts_int = check_if_code_consumes_fixed_time hd ts in
@@ -177,7 +177,7 @@ let rec check_if_block_consumes_fixed_time (block:tainted_codes) (ts:taintState)
     else check_if_block_consumes_fixed_time tl ts_int
 
 
-and check_if_code_consumes_fixed_time (code:tainted_code) (ts:taintState) : bool * taintState =
+and check_if_code_consumes_fixed_time (code:tainted_code) (ts:analysis_taints) : bool * analysis_taints =
   match code with
   | Ins ins -> check_if_ins_consumes_fixed_time ins ts
 
@@ -206,7 +206,7 @@ and check_if_code_consumes_fixed_time (code:tainted_code) (ts:taintState) : bool
 
   | While cond body -> check_if_loop_consumes_fixed_time code ts
 
-and check_if_loop_consumes_fixed_time c (ts:taintState) : (bool * taintState) =
+and check_if_loop_consumes_fixed_time c (ts:analysis_taints) : (bool * analysis_taints) =
   let While pred body = c in
   let cond_taint = pred.ot in
   let o1 = operand_taint (get_fst_ocmp pred.o) ts Public in
@@ -232,16 +232,16 @@ and check_if_loop_consumes_fixed_time c (ts:taintState) : (bool * taintState) =
       check_if_loop_consumes_fixed_time c combined_ts
     )
 
-val monotone_ok_eval: (code:tainted_code) -> (fuel:nat) -> (s:traceState) -> Lemma
+val monotone_ok_eval: (code:tainted_code) -> (fuel:nat) -> (s:S.machine_state) -> Lemma
  (requires True)
  (ensures (let s' = taint_eval_code code fuel s in
-    Some? s' /\ (Some?.v s').state.S.ok ==> s.state.S.ok))
+    Some? s' /\ (Some?.v s').S.ms_ok ==> s.S.ms_ok))
  (decreases %[code; 0])
 
-val monotone_ok_eval_block: (codes:tainted_codes) -> (fuel:nat) -> (s:traceState) -> Lemma
+val monotone_ok_eval_block: (codes:tainted_codes) -> (fuel:nat) -> (s:S.machine_state) -> Lemma
  (requires True)
  (ensures (let s' = taint_eval_codes codes fuel s in
-    Some? s' /\ (Some?.v s').state.S.ok ==> s.state.S.ok))
+    Some? s' /\ (Some?.v s').S.ms_ok ==> s.S.ms_ok))
  (decreases %[codes;1])
 
 #set-options "--z3rlimit 20 --initial_ifuel 0 --max_ifuel 1 --initial_fuel 2 --max_fuel 2"
@@ -250,7 +250,7 @@ let rec monotone_ok_eval code fuel s = match code with
   | Block block -> monotone_ok_eval_block block fuel s
   | IfElse ifCond ifTrue ifFalse ->
     let st, b = taint_eval_ocmp s ifCond in
-    let st = {st with trace=BranchPredicate(b)::s.trace} in
+    let st = {st with S.ms_trace = BranchPredicate(b)::s.S.ms_trace} in
     if b then monotone_ok_eval ifTrue fuel st else monotone_ok_eval ifFalse fuel st
   | While cond body ->
     if fuel = 0 then ()
@@ -258,7 +258,7 @@ let rec monotone_ok_eval code fuel s = match code with
     let st, b = taint_eval_ocmp s cond in
     if not b then ()
     else
-    let st = {st with trace=BranchPredicate(b)::s.trace} in
+    let st = {st with S.ms_trace = BranchPredicate(b)::s.S.ms_trace} in
     monotone_ok_eval body (fuel-1) st;
     ()
 
@@ -271,13 +271,13 @@ and monotone_ok_eval_block block fuel s =
     monotone_ok_eval_block tl fuel (Some?.v s');
     monotone_ok_eval hd fuel s
 
-val monotone_ok_eval_while: (code:tainted_code{While? code}) -> (fuel:nat) -> (s:traceState) -> Lemma
+val monotone_ok_eval_while: (code:tainted_code{While? code}) -> (fuel:nat) -> (s:S.machine_state) -> Lemma
   (requires True)
   (ensures (
       let While cond body = code in
       let (s1, b1) = taint_eval_ocmp s cond in
       let r1 = taint_eval_code code fuel s in
-      Some? r1 /\ (Some?.v r1).state.S.ok ==> s1.state.S.ok))
+      Some? r1 /\ (Some?.v r1).S.ms_ok ==> s1.S.ms_ok))
 
 let monotone_ok_eval_while code fuel s =
   let While cond body = code in
@@ -285,18 +285,18 @@ let monotone_ok_eval_while code fuel s =
   let r1 = taint_eval_while code fuel s in
   if fuel = 0 then ()
   else if not b then ()
-  else let s0 = {s1 with trace = BranchPredicate(true)::s1.trace} in
+  else let s0 = {s1 with S.ms_trace = BranchPredicate(true)::s1.S.ms_trace} in
   let s_opt = taint_eval_code body (fuel - 1) s0 in
   match s_opt with
     | None -> ()
-    | Some s -> if not s.state.S.ok then ()
+    | Some s -> if not s.S.ms_ok then ()
       else monotone_ok_eval body (fuel -1) s0; monotone_ok_eval code (fuel - 1) s
 
-val lemma_loop_taintstate_monotone: (ts:taintState) -> (code:tainted_code{While? code}) -> Lemma
-(requires True)
-(ensures (let _, ts' = check_if_loop_consumes_fixed_time code ts in
-  taintstate_monotone ts ts'))
-(decreases %[count_publics ts])
+val lemma_loop_taintstate_monotone (ts:analysis_taints) (code:tainted_code{While? code}) : Lemma
+  (requires True)
+  (ensures (let _, ts' = check_if_loop_consumes_fixed_time code ts in
+    taintstate_monotone ts ts'))
+  (decreases %[count_publics ts])
 
 #reset-options "--initial_ifuel 1 --max_ifuel 1 --initial_fuel 2 --max_fuel 2 --z3rlimit 40"
 let rec lemma_loop_taintstate_monotone ts code =
@@ -312,35 +312,35 @@ let rec lemma_loop_taintstate_monotone ts code =
   )
 
 #reset-options "--initial_ifuel 1 --max_ifuel 1 --initial_fuel 2 --max_fuel 2 --z3rlimit 60"
-val lemma_code_explicit_leakage_free: (ts:taintState) -> (code:tainted_code) -> (s1:traceState) -> (s2:traceState) -> (fuel:nat) -> Lemma
- (requires True)
- (ensures (let b, ts' = check_if_code_consumes_fixed_time code ts in
-  (b2t b ==> isConstantTimeGivenStates code fuel ts s1 s2 /\ isExplicitLeakageFreeGivenStates code fuel ts ts' s1 s2)))
- (decreases %[fuel; code; 1])
+val lemma_code_explicit_leakage_free: (ts:analysis_taints) -> (code:tainted_code) -> (s1:S.machine_state) -> (s2:S.machine_state) -> (fuel:nat) -> Lemma
+  (requires True)
+  (ensures (let b, ts' = check_if_code_consumes_fixed_time code ts in
+    (b2t b ==> isConstantTimeGivenStates code fuel ts s1 s2 /\ isExplicitLeakageFreeGivenStates code fuel ts ts' s1 s2)))
+  (decreases %[fuel; code; 1])
 
-val lemma_block_explicit_leakage_free: (ts:taintState) -> (codes:tainted_codes) -> (s1:traceState) -> (s2:traceState) -> (fuel:nat) -> Lemma
- (requires True)
- (ensures (let b, ts' = check_if_block_consumes_fixed_time codes ts in
-  (b2t b ==> isConstantTimeGivenStates (Block codes) fuel ts s1 s2 /\ isExplicitLeakageFreeGivenStates (Block codes) fuel ts ts' s1 s2)))
- (decreases %[fuel; codes; 2])
+val lemma_block_explicit_leakage_free: (ts:analysis_taints) -> (codes:tainted_codes) -> (s1:S.machine_state) -> (s2:S.machine_state) -> (fuel:nat) -> Lemma
+  (requires True)
+  (ensures (let b, ts' = check_if_block_consumes_fixed_time codes ts in
+    (b2t b ==> isConstantTimeGivenStates (Block codes) fuel ts s1 s2 /\ isExplicitLeakageFreeGivenStates (Block codes) fuel ts ts' s1 s2)))
+  (decreases %[fuel; codes; 2])
 
-val lemma_loop_explicit_leakage_free: (ts:taintState) -> (code:tainted_code{While? code}) -> (s1:traceState) -> (s2:traceState) -> (fuel:nat) -> Lemma
- (requires True)
- (ensures (let b, ts' = check_if_loop_consumes_fixed_time code ts in
-  (b2t b ==> isConstantTimeGivenStates code fuel ts s1 s2 /\ isExplicitLeakageFreeGivenStates code fuel ts ts' s1 s2)))
- (decreases %[fuel; code; 0])
+val lemma_loop_explicit_leakage_free: (ts:analysis_taints) -> (code:tainted_code{While? code}) -> (s1:S.machine_state) -> (s2:S.machine_state) -> (fuel:nat) -> Lemma
+  (requires True)
+  (ensures (let b, ts' = check_if_loop_consumes_fixed_time code ts in
+    (b2t b ==> isConstantTimeGivenStates code fuel ts s1 s2 /\ isExplicitLeakageFreeGivenStates code fuel ts ts' s1 s2)))
+  (decreases %[fuel; code; 0])
 
 #reset-options "--initial_ifuel 2 --max_ifuel 2 --initial_fuel 1 --max_fuel 2 --z3rlimit 300"
- let rec lemma_code_explicit_leakage_free ts code s1 s2 fuel = match code with
+let rec lemma_code_explicit_leakage_free ts code s1 s2 fuel = match code with
   | Ins ins -> lemma_ins_leakage_free ts ins
   | Block block -> lemma_block_explicit_leakage_free ts block s1 s2 fuel
   | IfElse ifCond ifTrue ifFalse ->
     let b_fin, ts_fin = check_if_code_consumes_fixed_time code ts in
     let st1, b1 = taint_eval_ocmp s1 ifCond in
-    let st1 = {st1 with trace=BranchPredicate(b1)::s1.trace} in
+    let st1 = {st1 with S.ms_trace = BranchPredicate(b1)::s1.S.ms_trace} in
     let st2, b2 = taint_eval_ocmp s2 ifCond in
-    let st2 = {st2 with trace=BranchPredicate(b2)::s2.trace} in
-    assert (b2t b_fin ==> constTimeInvariant ts s1 s2 /\ st1.state.S.ok /\ st2.state.S.ok ==> constTimeInvariant ts st1 st2);
+    let st2 = {st2 with S.ms_trace = BranchPredicate(b2)::s2.S.ms_trace} in
+    assert (b2t b_fin ==> constTimeInvariant ts s1 s2 /\ st1.S.ms_ok /\ st2.S.ms_ok ==> constTimeInvariant ts st1 st2);
     monotone_ok_eval ifTrue fuel st1;
     monotone_ok_eval ifTrue fuel st2;
     lemma_code_explicit_leakage_free ts ifTrue st1 st2 fuel;
@@ -374,25 +374,25 @@ and lemma_loop_explicit_leakage_free ts code s1 s2 fuel =
   let (st1, b1) = taint_eval_ocmp s1 cond in
   let (st2, b2) = taint_eval_ocmp s2 cond in
 
-  assert (b2t b_fin ==> constTimeInvariant ts s1 s2 /\ st1.state.S.ok /\ st2.state.S.ok ==> b1 = b2);
-  assert (b2t b_fin ==> constTimeInvariant ts s1 s2 /\ st1.state.S.ok /\ st2.state.S.ok ==> constTimeInvariant ts st1 st2);
+  assert (b2t b_fin ==> constTimeInvariant ts s1 s2 /\ st1.S.ms_ok /\ st2.S.ms_ok ==> b1 = b2);
+  assert (b2t b_fin ==> constTimeInvariant ts s1 s2 /\ st1.S.ms_ok /\ st2.S.ms_ok ==> constTimeInvariant ts st1 st2);
   if not b1 || not b2 then
   (
-  assert (b2t b_fin ==> constTimeInvariant ts s1 s2 /\ st1.state.S.ok /\ st2.state.S.ok ==> not b1 /\ not b2);
-  assert (not b1 ==> r1 == Some ({st1 with trace = BranchPredicate(false)::st1.trace}));
-  assert (not b2 ==> r2 == Some ({st2 with trace = BranchPredicate(false)::st2.trace}));
+  assert (b2t b_fin ==> constTimeInvariant ts s1 s2 /\ st1.S.ms_ok /\ st2.S.ms_ok ==> not b1 /\ not b2);
+  assert (not b1 ==> r1 == Some ({st1 with S.ms_trace = BranchPredicate(false)::st1.S.ms_trace}));
+  assert (not b2 ==> r2 == Some ({st2 with S.ms_trace = BranchPredicate(false)::st2.S.ms_trace}));
   monotone_ok_eval_while code fuel s1;
-  assert (Some? r1 /\ (Some?.v r1).state.S.ok ==> st1.state.S.ok);
+  assert (Some? r1 /\ (Some?.v r1).S.ms_ok ==> st1.S.ms_ok);
   monotone_ok_eval_while code fuel s2;
-  assert (Some? r2 /\ (Some?.v r2).state.S.ok ==> st2.state.S.ok);
+  assert (Some? r2 /\ (Some?.v r2).S.ms_ok ==> st2.S.ms_ok);
   lemma_loop_taintstate_monotone ts code;
   isExplicit_monotone ts ts ts_fin code fuel s1 s2;
   ()
   )
   else
-  let st'1 = ({st1 with trace = BranchPredicate(true)::st1.trace}) in
-  let st'2 = ({st2 with trace = BranchPredicate(true)::st2.trace}) in
-  assert (b2t b_fin ==> constTimeInvariant ts s1 s2 /\ st'1.state.S.ok /\ st'2.state.S.ok ==> constTimeInvariant ts st'1 st'2);
+  let st'1 = ({st1 with S.ms_trace = BranchPredicate(true)::st1.S.ms_trace}) in
+  let st'2 = ({st2 with S.ms_trace = BranchPredicate(true)::st2.S.ms_trace}) in
+  assert (b2t b_fin ==> constTimeInvariant ts s1 s2 /\ st'1.S.ms_ok /\ st'2.S.ms_ok ==> constTimeInvariant ts st'1 st'2);
   let b', ts' = check_if_code_consumes_fixed_time body ts in
   lemma_code_explicit_leakage_free ts body st'1 st'2 (fuel-1);
   monotone_ok_eval body (fuel-1) st'1;
@@ -405,23 +405,23 @@ and lemma_loop_explicit_leakage_free ts code s1 s2 fuel =
   else
   let st1 = Some?.v st1 in
   let st2 = Some?.v st2 in
-  if not st1.state.S.ok || not st2.state.S.ok then ()
+  if not st1.S.ms_ok || not st2.S.ms_ok then ()
   else
   let combined_ts = combine_taint_states ts ts' in
   let b_aux, ts_aux = check_if_loop_consumes_fixed_time code combined_ts in
   lemma_loop_explicit_leakage_free combined_ts code st1 st2 (fuel-1);
   isConstant_monotone ts combined_ts code (fuel-1) st1 st2;
   isExplicit_monotone2 ts_aux ts combined_ts code (fuel-1) st1 st2;
-  assert (b2t b_fin ==> constTimeInvariant ts s1 s2 /\ st1.state.S.ok /\ st2.state.S.ok ==> constTimeInvariant ts' st1 st2)
+  assert (b2t b_fin ==> constTimeInvariant ts s1 s2 /\ st1.S.ms_ok /\ st2.S.ms_ok ==> constTimeInvariant ts' st1 st2)
 
-val lemma_code_leakage_free: (ts:taintState) -> (code:tainted_code) -> Lemma
+val lemma_code_leakage_free: (ts:analysis_taints) -> (code:tainted_code) -> Lemma
  (let b, ts' = check_if_code_consumes_fixed_time code ts in
   (b2t b ==> isConstantTime code ts /\ isLeakageFree code ts ts'))
 
 let lemma_code_leakage_free ts code = FStar.Classical.forall_intro_3 (lemma_code_explicit_leakage_free ts code)
 
 #set-options "--z3rlimit 20"
-val check_if_code_is_leakage_free: (code:tainted_code) -> (ts:taintState) -> (tsExpected:taintState) -> (b:bool{b ==> isLeakageFree code ts tsExpected
+val check_if_code_is_leakage_free: (code:tainted_code) -> (ts:analysis_taints) -> (tsExpected:analysis_taints) -> (b:bool{b ==> isLeakageFree code ts tsExpected
          /\ b ==> isConstantTime code ts})
 
 let check_if_code_is_leakage_free code ts tsExpected =
