vale/code/arch/x64/X64.Leakage_Helpers.fst
@@ -16,7 +16,7 @@ let operand_taint (op:operand) ts taint =
     | OReg reg -> ts.regTaint reg
     | OMem _ | OStack _ -> taint
 
-let operand_taint128 (op:mov128_op) (ts:taintState) (t:taint) : taint =
+let operand_taint128 (op:mov128_op) (ts:analysis_taints) (t:taint) : taint =
   match op with
   | Mov128Xmm x -> ts.xmmTaint x
   | Mov128Mem _ | Mov128Stack _ -> t
@@ -25,7 +25,7 @@ let operand_taint128 (op:mov128_op) (ts:taintState) (t:taint) : taint =
 let operand_taint_explicit
   (i:instr_operand_explicit)
   (o:instr_operand_t i)
-  (ts:taintState)
+  (ts:analysis_taints)
   (t:taint) : taint =
   match i with
   | IOp64 -> operand_taint o ts t
@@ -34,7 +34,7 @@ let operand_taint_explicit
 [@instr_attr]
 let operand_taint_implicit
   (i:instr_operand_implicit)
-  (ts:taintState)
+  (ts:analysis_taints)
   (t:taint) : taint =
   match i with
   | IOp64One o -> operand_taint o ts t
@@ -46,7 +46,7 @@ let operand_taint_implicit
 let rec args_taint
   (args:list instr_operand)
   (oprs:instr_operands_t_args args)
-  (ts:taintState)
+  (ts:analysis_taints)
   (t:taint) : taint =
   match args with
   | [] -> Public
@@ -64,7 +64,7 @@ let rec inouts_taint
   (inouts:list instr_out) 
   (args:list instr_operand)
   (oprs:instr_operands_t inouts args)
-  (ts:taintState)
+  (ts:analysis_taints)
   (t:taint) : taint =
   match inouts with
   | [] -> args_taint args oprs ts t
@@ -97,7 +97,7 @@ let operand_does_not_use_secrets op ts =
   | OConst _ | OReg _ -> true 
   | OMem m | OStack m -> maddr_does_not_use_secrets m ts
 
-let operand128_does_not_use_secrets (op:mov128_op) (ts:taintState) : bool =
+let operand128_does_not_use_secrets (op:mov128_op) (ts:analysis_taints) : bool =
   match op with
   | Mov128Xmm _ -> true
   | Mov128Mem m | Mov128Stack m -> maddr_does_not_use_secrets m ts
@@ -112,7 +112,7 @@ let operand128_taint_allowed (o:mov128_op) (t_operand t_data:taint) : bool =
   | Mov128Xmm _ -> true
   | Mov128Mem _ | Mov128Stack _ -> t_operand = Secret || t_data = Public
 
-val lemma_operand_obs:  (ts:taintState) ->  (dst:operand) -> (s1 : traceState) -> (s2:traceState) -> Lemma ((operand_does_not_use_secrets dst ts) /\ publicValuesAreSame ts s1 s2 ==> (operand_obs s1 dst) = (operand_obs s2 dst))
+val lemma_operand_obs:  (ts:analysis_taints) ->  (dst:operand) -> (s1 : machine_state) -> (s2:machine_state) -> Lemma ((operand_does_not_use_secrets dst ts) /\ publicValuesAreSame ts s1 s2 ==> (operand_obs s1 dst) = (operand_obs s2 dst))
 
 #reset-options "--initial_ifuel 2 --max_ifuel 2 --initial_fuel 4 --max_fuel 4 --z3rlimit 20"
 let lemma_operand_obs ts dst s1 s2 = match dst with
@@ -120,43 +120,43 @@ let lemma_operand_obs ts dst s1 s2 = match dst with
   | OMem m | OStack m  -> ()
 #reset-options "--initial_ifuel 2 --max_ifuel 2 --initial_fuel 4 --max_fuel 4 --z3rlimit 5"
 
-let set_taint (dst:operand) ts taint : Tot taintState =
+let set_taint (dst:operand) ts taint : Tot analysis_taints =
   match dst with
   | OConst _ -> ts  (* Shouldn't actually happen *)
-  | OReg r -> TaintState (FunctionalExtensionality.on reg (fun x -> if x = r then taint else ts.regTaint x)) ts.flagsTaint ts.cfFlagsTaint ts.ofFlagsTaint ts.xmmTaint
+  | OReg r -> AnalysisTaints (FunctionalExtensionality.on reg (fun x -> if x = r then taint else ts.regTaint x)) ts.flagsTaint ts.cfFlagsTaint ts.ofFlagsTaint ts.xmmTaint
   | OMem m | OStack m -> ts (* Ensured by taint semantics *)
 
-let set_taint128 (dst:mov128_op) (ts:taintState) (t:taint) : taintState =
+let set_taint128 (dst:mov128_op) (ts:analysis_taints) (t:taint) : analysis_taints =
   match dst with
-  | Mov128Xmm r -> TaintState ts.regTaint ts.flagsTaint ts.cfFlagsTaint ts.ofFlagsTaint
+  | Mov128Xmm r -> AnalysisTaints ts.regTaint ts.flagsTaint ts.cfFlagsTaint ts.ofFlagsTaint
       (FunctionalExtensionality.on xmm (fun x -> if x = r then t else ts.xmmTaint x))
   | Mov128Mem _ | Mov128Stack _-> ts
 
-let set_taint_cf_and_flags (ts:taintState) (t:taint) : taintState =
-  let TaintState rs flags cf ovf xmms = ts in
-  TaintState rs (merge_taint t flags) t ovf xmms
+let set_taint_cf_and_flags (ts:analysis_taints) (t:taint) : analysis_taints =
+  let AnalysisTaints rs flags cf ovf xmms = ts in
+  AnalysisTaints rs (merge_taint t flags) t ovf xmms
 
-let set_taint_of_and_flags (ts:taintState) (t:taint) : taintState =
-  let TaintState rs flags cf ovf xmms = ts in
-  TaintState rs (merge_taint t flags) cf t xmms
+let set_taint_of_and_flags (ts:analysis_taints) (t:taint) : analysis_taints =
+  let AnalysisTaints rs flags cf ovf xmms = ts in
+  AnalysisTaints rs (merge_taint t flags) cf t xmms
 
 let rec operands_do_not_use_secrets ops ts = match ops with
   | [] -> true
   | hd :: tl -> operand_does_not_use_secrets hd ts && (operands_do_not_use_secrets tl ts)
 
-val lemma_operands_imply_op: (ts:taintState) -> (ops:list operand{Cons? ops}) -> Lemma
-(requires (operands_do_not_use_secrets ops ts))
-(ensures (operand_does_not_use_secrets (List.Tot.Base.hd ops) ts))
+val lemma_operands_imply_op: (ts:analysis_taints) -> (ops:list operand{Cons? ops}) -> Lemma
+  (requires (operands_do_not_use_secrets ops ts))
+  (ensures (operand_does_not_use_secrets (List.Tot.Base.hd ops) ts))
 
 let lemma_operands_imply_op ts ops = match ops with
-| hd :: tl -> ()
+  | hd :: tl -> ()
 
-let ins_consumes_fixed_time (ins : tainted_ins) (ts:taintState) (res:bool*taintState) =
+let ins_consumes_fixed_time (ins : tainted_ins) (ts:analysis_taints) (res:bool*analysis_taints) =
   let b, ts' = res in
   ((b2t b) ==> isConstantTime (Ins ins) ts)
 
 
-(*val lemma_operand_obs_list: (ts:taintState) -> (ops:list operand) -> (s1:traceState) -> (s2:traceState) -> Lemma  ((operands_do_not_use_secrets ops ts /\ publicValuesAreSame ts s1 s2) ==>
+(*val lemma_operand_obs_list: (ts:analysis_taints) -> (ops:list operand) -> (s1:machine_state) -> (s2:machine_state) -> Lemma  ((operands_do_not_use_secrets ops ts /\ publicValuesAreSame ts s1 s2) ==>
   (operand_obs_list s1 ops) == (operand_obs_list s2 ops))
 
 let rec lemma_operand_obs_list ts ops s1 s2 = match ops with
@@ -172,7 +172,7 @@ let rec set_taints dsts ts taint = match dsts with
   | [] -> ts
   | hd :: tl -> set_taints tl (set_taint hd ts taint) taint
 
-val lemma_taint_sources: (ins:tainted_ins) -> (ts:taintState) -> Lemma
+val lemma_taint_sources: (ins:tainted_ins) -> (ts:analysis_taints) -> Lemma
 (let i = ins.i in
  let d, s = extract_operands i in
 forall src. List.Tot.Base.mem src s /\ Public? (sources_taint s ts ins.t) ==> Public? (operand_taint src ts ins.t))
@@ -182,47 +182,47 @@ let lemma_taint_sources ins ts = ()
 #set-options "--z3rlimit 20"
 
 val lemma_public_op_are_same:
-  (ts:taintState) -> (op:operand) -> (s1:traceState) -> (s2:traceState)
+  (ts:analysis_taints) -> (op:operand) -> (s1:machine_state) -> (s2:machine_state)
    -> Lemma (requires (operand_does_not_use_secrets op ts   /\
                       Public? (operand_taint op ts Public) /\
 		      publicValuesAreSame ts s1 s2         /\
-		      taint_match op Public s1.memTaint s1.stackTaint s1.state /\
-		      taint_match op Public s2.memTaint s2.stackTaint s2.state))
-           (ensures eval_operand op s1.state == eval_operand op s2.state)
+		      taint_match op Public s1.ms_memTaint s1.ms_stackTaint s1 /\
+		      taint_match op Public s2.ms_memTaint s2.ms_stackTaint s2))
+           (ensures eval_operand op s1 == eval_operand op s2)
 let lemma_public_op_are_same ts op s1 s2 =
   match op with
   | OConst _ -> ()
   | OReg _ -> ()
   | OMem m | OStack m ->
-    let a1 = eval_maddr m s1.state in
-    let a2 = eval_maddr m s2.state in
+    let a1 = eval_maddr m s1 in
+    let a2 = eval_maddr m s2 in
     assert (a1 == a2);
-//    assert (forall a. (a >= a1 /\ a < a1 + 8) ==> s1.state.mem.[a] == s2.state.mem.[a]);
+//    assert (forall a. (a >= a1 /\ a < a1 + 8) ==> s1.ms_mem.[a] == s2.ms_mem.[a]);
     Opaque_s.reveal_opaque get_heap_val64_def
 
-val publicFlagValuesAreAsExpected: (tsAnalysis:taintState) -> (tsExpected:taintState) -> b:bool{b <==> (Public? tsExpected.flagsTaint ==> Public? tsAnalysis.flagsTaint)}
+val publicFlagValuesAreAsExpected: (tsAnalysis:analysis_taints) -> (tsExpected:analysis_taints) -> b:bool{b <==> (Public? tsExpected.flagsTaint ==> Public? tsAnalysis.flagsTaint)}
 
-val publicCfFlagValuesAreAsExpected: (tsAnalysis:taintState) -> (tsExpected:taintState) -> b:bool{b <==> (Public? tsExpected.cfFlagsTaint ==> Public? tsAnalysis.cfFlagsTaint)}
+val publicCfFlagValuesAreAsExpected: (tsAnalysis:analysis_taints) -> (tsExpected:analysis_taints) -> b:bool{b <==> (Public? tsExpected.cfFlagsTaint ==> Public? tsAnalysis.cfFlagsTaint)}
 
-val publicOfFlagValuesAreAsExpected: (tsAnalysis:taintState) -> (tsExpected:taintState) -> b:bool{b <==> (Public? tsExpected.ofFlagsTaint ==> Public? tsAnalysis.ofFlagsTaint)}
+val publicOfFlagValuesAreAsExpected: (tsAnalysis:analysis_taints) -> (tsExpected:analysis_taints) -> b:bool{b <==> (Public? tsExpected.ofFlagsTaint ==> Public? tsAnalysis.ofFlagsTaint)}
 
-val publicRegisterValuesAreAsExpected: (tsAnalysis:taintState) -> (tsExpected:taintState) -> b:bool{b <==> (forall r. (Public? (tsExpected.regTaint r) ==> Public? (tsAnalysis.regTaint r)))}
+val publicRegisterValuesAreAsExpected: (tsAnalysis:analysis_taints) -> (tsExpected:analysis_taints) -> b:bool{b <==> (forall r. (Public? (tsExpected.regTaint r) ==> Public? (tsAnalysis.regTaint r)))}
 
-val publicTaintsAreAsExpected: (tsAnalysis:taintState) -> (tsExpected:taintState) -> b:bool
+val publicTaintsAreAsExpected: (tsAnalysis:analysis_taints) -> (tsExpected:analysis_taints) -> b:bool
 
-let publicFlagValuesAreAsExpected (tsAnalysis:taintState) (tsExpected:taintState) =
+let publicFlagValuesAreAsExpected (tsAnalysis:analysis_taints) (tsExpected:analysis_taints) =
   (tsExpected.flagsTaint = Public && tsAnalysis.flagsTaint = Public) || (tsExpected.flagsTaint = Secret)
 
-let publicCfFlagValuesAreAsExpected (tsAnalysis:taintState) (tsExpected:taintState) =
+let publicCfFlagValuesAreAsExpected (tsAnalysis:analysis_taints) (tsExpected:analysis_taints) =
   (tsExpected.cfFlagsTaint = Public && tsAnalysis.cfFlagsTaint = Public) || (tsExpected.cfFlagsTaint = Secret)
 
-let publicOfFlagValuesAreAsExpected (tsAnalysis:taintState) (tsExpected:taintState) =
+let publicOfFlagValuesAreAsExpected (tsAnalysis:analysis_taints) (tsExpected:analysis_taints) =
   (tsExpected.ofFlagsTaint = Public && tsAnalysis.ofFlagsTaint = Public) || (tsExpected.ofFlagsTaint = Secret)
 
-let registerAsExpected (r:reg) (tsAnalysis:taintState) (tsExpected:taintState) =
+let registerAsExpected (r:reg) (tsAnalysis:analysis_taints) (tsExpected:analysis_taints) =
   (tsExpected.regTaint r = Public && tsAnalysis.regTaint r = Public) || (tsExpected.regTaint r = Secret)
 
-let publicRegisterValuesAreAsExpected (tsAnalysis:taintState) (tsExpected:taintState) =
+let publicRegisterValuesAreAsExpected (tsAnalysis:analysis_taints) (tsExpected:analysis_taints) =
   registerAsExpected rRax tsAnalysis tsExpected &&
   registerAsExpected rRbx tsAnalysis tsExpected &&
   registerAsExpected rRcx tsAnalysis tsExpected &&
@@ -240,7 +240,7 @@ let publicRegisterValuesAreAsExpected (tsAnalysis:taintState) (tsExpected:taintS
   registerAsExpected rR14 tsAnalysis tsExpected &&
   registerAsExpected rR15 tsAnalysis tsExpected
 
-let publicTaintsAreAsExpected (tsAnalysis:taintState) (tsExpected:taintState) =
+let publicTaintsAreAsExpected (tsAnalysis:analysis_taints) (tsExpected:analysis_taints) =
     publicFlagValuesAreAsExpected tsAnalysis tsExpected
   && publicCfFlagValuesAreAsExpected tsAnalysis tsExpected
   && publicOfFlagValuesAreAsExpected tsAnalysis tsExpected
