vale/code/arch/x64/X64.Leakage_Ins.fst
@@ -13,10 +13,10 @@ let rec has_mem_operand = function
   | a::q -> if OMem? a || OStack? a then true else has_mem_operand q
 
 let rec check_if_consumes_fixed_time_args
-    (args:list instr_operand) (oprs:instr_operands_t_args args) (ts:taintState)
+    (args:list instr_operand) (oprs:instr_operands_t_args args) (ts:analysis_taints)
   : Pure bool
     (requires True)
-    (ensures fun b -> b ==> (forall (s1 s2:traceState).{:pattern (constTimeInvariant ts s1 s2)}
+    (ensures fun b -> b ==> (forall (s1 s2:S.machine_state).{:pattern (constTimeInvariant ts s1 s2)}
       constTimeInvariant ts s1 s2 ==> obs_args args oprs s1 == obs_args args oprs s2))
   =
   match args with
@@ -49,61 +49,73 @@ let rec check_if_consumes_fixed_time_args
     let b'' = check_if_consumes_fixed_time_args args (coerce oprs) ts in
     b' && b''
 
+let check_if_consumes_fixed_time_outs_explicit
+    (i:instr_operand_explicit) (o:instr_operand_t i)
+    (ts:analysis_taints) (t_ins t_out:taint)
+  : bool
+  =
+  match i with
+  | IOp64 -> operand_does_not_use_secrets o ts && operand_taint_allowed o t_ins t_out
+  | IOpXmm -> operand128_does_not_use_secrets o ts && operand128_taint_allowed o t_ins t_out
+
+let check_if_consumes_fixed_time_outs_implicit
+    (i:instr_operand_implicit) (ts:analysis_taints) (t_ins t_out:taint)
+  : bool
+  =
+  match i with
+  | IOp64One o -> operand_does_not_use_secrets o ts && operand_taint_allowed o t_ins t_out
+  | IOpXmmOne o -> operand128_does_not_use_secrets o ts && operand128_taint_allowed o t_ins t_out
+  | IOpFlagsCf -> true
+  | IOpFlagsOf -> true
+
 let rec check_if_consumes_fixed_time_outs
     (outs:list instr_out) (args:list instr_operand) (oprs:instr_operands_t outs args)
-    (ts:taintState) (t_ins t_out:taint)
+    (ts:analysis_taints) (t_ins t_out:taint)
   : Pure bool
     (requires True)
-    (ensures fun b -> b ==> (forall (s1 s2:traceState).{:pattern (constTimeInvariant ts s1 s2)}
+    (ensures fun b -> b ==> (forall (s1 s2:S.machine_state).{:pattern (constTimeInvariant ts s1 s2)}
       constTimeInvariant ts s1 s2 ==> obs_inouts outs args oprs s1 == obs_inouts outs args oprs s2))
   =
   match outs with
   | [] -> check_if_consumes_fixed_time_args args oprs ts
   | (_, IOpEx i)::outs ->
     let ((o:instr_operand_t i), (oprs:instr_operands_t outs args)) = coerce oprs in
-    let b' =
+    let o =
       match i with
-      | IOp64 ->
-        let o = match coerce o with | OMem _ | OStack _ -> o | _ -> o in
-        operand_does_not_use_secrets o ts && operand_taint_allowed o t_ins t_out
-      | IOpXmm ->
-        let o = match coerce o with | Mov128Mem _ | Mov128Stack _ | _ -> o in
-        operand128_does_not_use_secrets o ts && operand128_taint_allowed o t_ins t_out
+      | IOp64 -> (match coerce o with | OMem _ | OStack _ -> o | _ -> o)
+      | IOpXmm -> (match coerce o with | Mov128Mem _ | Mov128Stack _ | _ -> o)
       in
+    let b' = check_if_consumes_fixed_time_outs_explicit i o ts t_ins t_out in
     let b'' = check_if_consumes_fixed_time_outs outs args oprs ts t_ins t_out in
     b' && b''
   | (_, IOpIm i)::outs ->
-    let b' =
+    let i =
       match i with
-      | IOp64One o ->
-        let o = match coerce o with | OMem _ | OStack _ -> o | _ -> o in
-        operand_does_not_use_secrets o ts && operand_taint_allowed o t_ins t_out
-      | IOpXmmOne o ->
-        let o = match coerce o with | Mov128Mem _ | Mov128Stack _ | _ -> o in
-        operand128_does_not_use_secrets o ts && operand128_taint_allowed o t_ins t_out
-      | IOpFlagsCf -> true
-      | IOpFlagsOf -> true
+      | IOp64One o -> IOp64One (match coerce o with | OMem _ | OStack _ -> o | _ -> o)
+      | IOpXmmOne o -> IOpXmmOne (match coerce o with | Mov128Mem _ | Mov128Stack _ | _ -> o)
+      | _ -> i
       in
+    let b' = check_if_consumes_fixed_time_outs_implicit i ts t_ins t_out in
     let b'' = check_if_consumes_fixed_time_outs outs args (coerce oprs) ts t_ins t_out in
     b' && b''
 
-#reset-options "--z3rlimit 100"
+#reset-options "--z3rlimit 80"
 let rec lemma_args_taint
     (outs:list instr_out) (args:list instr_operand)
     (f:instr_args_t outs args) (oprs:instr_operands_t_args args)
-    (ts:taintState) (t_ins:taint) (s1 s2:traceState)
+    (ts:analysis_taints) (t_ins:taint) (s1 s2:S.machine_state)
   : Lemma
     (requires
       constTimeInvariant ts s1 s2 /\
-      taint_match_args args oprs t_ins s1.memTaint s1.stackTaint s1.state /\
-      taint_match_args args oprs t_ins s2.memTaint s2.stackTaint s2.state /\
-      Some? (S.instr_apply_eval_args outs args f oprs s1.state) /\
-      Some? (S.instr_apply_eval_args outs args f oprs s2.state) /\
+      taint_match_args args oprs t_ins s1.S.ms_memTaint s1.S.ms_stackTaint s1 /\
+      taint_match_args args oprs t_ins s2.S.ms_memTaint s2.S.ms_stackTaint s2 /\
+      Some? (S.instr_apply_eval_args outs args f oprs s1) /\
+      Some? (S.instr_apply_eval_args outs args f oprs s2) /\
       check_if_consumes_fixed_time_args args oprs ts /\
       args_taint args oprs ts t_ins == Public)
     (ensures
-      S.instr_apply_eval_args outs args f oprs s1.state ==
-      S.instr_apply_eval_args outs args f oprs s2.state)
+      S.instr_apply_eval_args outs args f oprs s1 ==
+      S.instr_apply_eval_args outs args f oprs s2)
   =
   match args with
   | [] -> ()
@@ -113,13 +125,13 @@ let rec lemma_args_taint
       match i with
       | IOpEx i ->
         let oprs = coerce oprs in (
-          S.instr_eval_operand_explicit i (fst oprs) s1.state,
-          S.instr_eval_operand_explicit i (fst oprs) s2.state,
+          S.instr_eval_operand_explicit i (fst oprs) s1,
+          S.instr_eval_operand_explicit i (fst oprs) s2,
           snd oprs)
       | IOpIm i ->
         let oprs = coerce oprs in (
-          S.instr_eval_operand_implicit i s1.state,
-          S.instr_eval_operand_implicit i s2.state,
+          S.instr_eval_operand_implicit i s1,
+          S.instr_eval_operand_implicit i s2,
           oprs)
       in
     let f:arrow (instr_val_t i) (instr_args_t outs args) = coerce f in
@@ -133,19 +145,19 @@ let rec lemma_args_taint
 let rec lemma_inouts_taint
     (outs inouts:list instr_out) (args:list instr_operand)
     (f:instr_inouts_t outs inouts args) (oprs:instr_operands_t inouts args)
-    (ts:taintState) (t_ins:taint) (s1 s2:traceState)
+    (ts:analysis_taints) (t_ins:taint) (s1 s2:S.machine_state)
   : Lemma
     (requires
       constTimeInvariant ts s1 s2 /\
-      taint_match_inouts inouts args oprs t_ins s1.memTaint s1.stackTaint s1.state /\
-      taint_match_inouts inouts args oprs t_ins s2.memTaint s2.stackTaint s2.state /\
-      Some? (S.instr_apply_eval_inouts outs inouts args f oprs s1.state) /\
-      Some? (S.instr_apply_eval_inouts outs inouts args f oprs s2.state) /\
+      taint_match_inouts inouts args oprs t_ins s1.S.ms_memTaint s1.S.ms_stackTaint s1 /\
+      taint_match_inouts inouts args oprs t_ins s2.S.ms_memTaint s2.S.ms_stackTaint s2 /\
+      Some? (S.instr_apply_eval_inouts outs inouts args f oprs s1) /\
+      Some? (S.instr_apply_eval_inouts outs inouts args f oprs s2) /\
       check_if_consumes_fixed_time_outs inouts args oprs ts t_ins Public /\
       inouts_taint inouts args oprs ts t_ins == Public)
     (ensures
-      S.instr_apply_eval_inouts outs inouts args f oprs s1.state ==
-      S.instr_apply_eval_inouts outs inouts args f oprs s2.state)
+      S.instr_apply_eval_inouts outs inouts args f oprs s1 ==
+      S.instr_apply_eval_inouts outs inouts args f oprs s2)
   =
   match inouts with
   | [] -> lemma_args_taint outs args f oprs ts t_ins s1 s2
@@ -162,13 +174,13 @@ let rec lemma_inouts_taint
       match i with
       | IOpEx i ->
         let oprs = coerce oprs in (
-          S.instr_eval_operand_explicit i (fst oprs) s1.state,
-          S.instr_eval_operand_explicit i (fst oprs) s2.state,
+          S.instr_eval_operand_explicit i (fst oprs) s1,
+          S.instr_eval_operand_explicit i (fst oprs) s2,
           snd oprs)
       | IOpIm i ->
         let oprs = coerce oprs in (
-          S.instr_eval_operand_implicit i s1.state,
-          S.instr_eval_operand_implicit i s2.state,
+          S.instr_eval_operand_implicit i s1,
+          S.instr_eval_operand_implicit i s2,
           oprs)
       in
     let f:arrow (instr_val_t i) (instr_inouts_t outs inouts args) = coerce f in
@@ -180,14 +192,14 @@ let rec lemma_inouts_taint
     lemma_inouts_taint outs inouts args (f v) oprs ts t_ins s1 s2
 
 let instr_set_taint_explicit
-    (i:instr_operand_explicit) (o:instr_operand_t i) (ts:taintState) (t:taint)
-  : taintState =
+    (i:instr_operand_explicit) (o:instr_operand_t i) (ts:analysis_taints) (t:taint)
+  : analysis_taints =
   match i with
   | IOp64 -> set_taint o ts t
   | IOpXmm -> set_taint128 o ts t
 
 [@instr_attr]
-let instr_set_taint_implicit (i:instr_operand_implicit) (ts:taintState) (t:taint) : taintState =
+let instr_set_taint_implicit (i:instr_operand_implicit) (ts:analysis_taints) (t:taint) : analysis_taints =
   match i with
   | IOp64One o -> set_taint o ts t
   | IOpXmmOne o -> set_taint128 o ts t
@@ -196,8 +208,8 @@ let instr_set_taint_implicit (i:instr_operand_implicit) (ts:taintState) (t:taint
 
 let rec instr_set_taints
     (outs:list instr_out) (args:list instr_operand)
-    (oprs:instr_operands_t outs args) (ts:taintState) (t:taint)
-  : taintState =
+    (oprs:instr_operands_t outs args) (ts:analysis_taints) (t:taint)
+  : analysis_taints =
   match outs with
   | [] -> ts
   | (_, i)::outs ->
@@ -211,10 +223,10 @@ let rec instr_set_taints
 
 let rec lemma_instr_write_outputs_ok
     (outs:list instr_out) (args:list instr_operand)
-    (vs:instr_ret_t outs) (oprs:instr_operands_t outs args) (s_orig s:S.state)
+    (vs:instr_ret_t outs) (oprs:instr_operands_t outs args) (s_orig s:S.machine_state)
   : Lemma
-    (requires (S.instr_write_outputs outs args vs oprs s_orig s).S.ok)
-    (ensures s.S.ok)
+    (requires (S.instr_write_outputs outs args vs oprs s_orig s).S.ms_ok)
+    (ensures s.S.ms_ok)
   =
   match outs with
   | [] -> ()
@@ -265,7 +277,7 @@ let lemma_update_heap32_val (ptr:int) (v:Types_s.nat32) (mem:S.heap) (i:int) : L
 let lemma_update_heap32_domain (ptr:int) (v:Types_s.nat32) (mem:S.heap) : Lemma
   (requires valid_addr32 ptr mem)
   (ensures Map.domain (S.update_heap32 ptr v mem) == Map.domain mem)
-  [SMTPat (S.update_heap32 ptr v mem)]
+  [SMTPat (Map.domain (S.update_heap32 ptr v mem))]
   =
   Opaque_s.reveal_opaque S.update_heap32_def;
   assert (Set.equal (Map.domain (S.update_heap32 ptr v mem)) (Map.domain mem))
@@ -289,13 +301,12 @@ let update_heap64_val (ptr:int) (v:nat64) (i:int) : Types_s.nat8 =
   | 7 -> hi.hi3
   | _ -> 0
 
-// TODO: this and lemma_update_heap32_val are convenient,
-// but they make lemma_instr_set_taints_* slow to verify.
-// Consider writing lemma_instr_set_taints_* in a more manual style.
 let lemma_update_heap64_val (ptr:int) (v:nat64) (mem:S.heap) (i:int) : Lemma
   (requires True)
-  (ensures (S.update_heap64 ptr v mem).[i] ==
-    (if ptr <= i && i < ptr + 8 then update_heap64_val ptr v i else mem.[i]))
+  (ensures
+    (S.update_heap64 ptr v mem).[i] ==
+    (if ptr <= i && i < ptr + 8 then update_heap64_val ptr v i else mem.[i])
+  )
   [SMTPat ((S.update_heap64 ptr v mem).[i])]
   =
   Opaque_s.reveal_opaque S.update_heap64_def;
@@ -304,43 +315,191 @@ let lemma_update_heap64_val (ptr:int) (v:nat64) (mem:S.heap) (i:int) : Lemma
 let lemma_update_heap64_domain (ptr:int) (v:nat64) (mem:S.heap) : Lemma
   (requires S.valid_addr64 ptr mem)
   (ensures Map.domain (S.update_heap64 ptr v mem) == Map.domain mem)
-  [SMTPat (S.update_heap64 ptr v mem)]
+  [SMTPat (Map.domain (S.update_heap64 ptr v mem))]
   =
+  FStar.Pervasives.reveal_opaque (`%S.valid_addr64) S.valid_addr64;
   Opaque_s.reveal_opaque S.update_heap64_def;
   assert (Set.equal (Map.domain (S.update_heap64 ptr v mem)) (Map.domain mem))
 
-#reset-options "--z3rlimit 1000"
-let rec lemma_instr_set_taints_secret
-    (outs:list instr_out) (args:list instr_operand)
-    (vs1 vs2:instr_ret_t outs) (oprs:instr_operands_t outs args) (ts_orig ts:taintState) (t_ins t_out:taint)
-    (s1_orig s1 s2_orig s2:traceState)
+[@"opaque_to_smt"]
+let update_heap128_val (ptr:int) (v:Types_s.quad32) (i:int) : Types_s.nat8 =
+  let open Words_s in
+  let j = i - ptr in
+  if  0 <= j && j <  4 then update_heap32_val (ptr + 0 ) v.lo0 i else
+  if  4 <= j && j <  8 then update_heap32_val (ptr + 4 ) v.lo1 i else
+  if  8 <= j && j < 12 then update_heap32_val (ptr + 8 ) v.hi2 i else
+  if 12 <= j && j < 16 then update_heap32_val (ptr + 12) v.hi3 i else
+  0
+
+let valid_addr128 (ptr:int) (mem:S.heap) : bool =
+  valid_addr32 (ptr + 0) mem &&
+  valid_addr32 (ptr + 4) mem &&
+  valid_addr32 (ptr + 8) mem &&
+  valid_addr32 (ptr + 12) mem
+
+let lemma_update_heap128_val (ptr:int) (v:Types_s.quad32) (mem:S.heap) (i:int) : Lemma
+  (requires True)
+  (ensures
+    (S.update_heap128 ptr v mem).[i] ==
+    (if ptr <= i && i < ptr + 16 then update_heap128_val ptr v i else mem.[i])
+  )
+  [SMTPat ((S.update_heap128 ptr v mem).[i])]
+  =
+  Opaque_s.reveal_opaque S.update_heap128_def;
+  FStar.Pervasives.reveal_opaque (`%update_heap128_val) update_heap128_val
+
+let lemma_update_heap128_domain (ptr:int) (v:Types_s.quad32) (mem:S.heap) : Lemma
+  (requires valid_addr128 ptr mem)
+  (ensures Map.domain (S.update_heap128 ptr v mem) == Map.domain mem)
+  [SMTPat (S.update_heap128 ptr v mem)]
+  =
+  Opaque_s.reveal_opaque S.update_heap128_def;
+  assert (Set.equal (Map.domain (S.update_heap128 ptr v mem)) (Map.domain mem))
+
+let lemma_preserve_valid64 (m m':S.heap) : Lemma
+  (requires Set.equal (Map.domain m) (Map.domain m'))
+  (ensures (forall (i:int).{:pattern (S.valid_addr64 i m')}
+    S.valid_addr64 i m ==> S.valid_addr64 i m'))
+  =
+  FStar.Pervasives.reveal_opaque (`%S.valid_addr64) S.valid_addr64
+
+let lemma_preserve_valid128 (m m':S.heap) : Lemma
+  (requires Set.equal (Map.domain m) (Map.domain m'))
+  (ensures (forall (i:int).{:pattern (S.valid_addr128 i m')}
+    S.valid_addr128 i m ==> S.valid_addr128 i m'))
+  =
+  FStar.Pervasives.reveal_opaque (`%S.valid_addr128) S.valid_addr128
+
+// Avoid extra ifuel for "with":
+let state_with_taint (s:S.machine_state) (memTaint stackTaint:memTaint_t) : Pure S.machine_state
+  (requires True)
+  (ensures fun s' ->
+    s'.S.ms_mem == s.S.ms_mem /\ s'.S.ms_stack == s.S.ms_stack /\
+    s'.S.ms_regs == s.S.ms_regs /\ s'.S.ms_xmms == s.S.ms_xmms)
+  =
+  {s with S.ms_memTaint = memTaint; S.ms_stackTaint = stackTaint}
+
+let lemma_instr_set_taints_explicit
+    (i:instr_operand_explicit) (v1 v2:instr_val_t (IOpEx i)) (o:instr_operand_t i)
+    (ts_orig ts:analysis_taints) (t_ins t_out:taint)
+    (s1_orig s1 s2_orig s2:S.machine_state)
+    (memTaint1 stackTaint1 memTaint2 stackTaint2:memTaint_t)
   : Lemma
     (requires (
-      let s1_state' = S.instr_write_outputs outs args vs1 oprs s1_orig.state s1.state in
-      let s2_state' = S.instr_write_outputs outs args vs2 oprs s2_orig.state s2.state in
-      s1_state'.S.ok /\ s2_state'.S.ok /\
-      t_out == Secret /\
-      Set.equal (Map.domain s1_orig.state.S.mem) (Map.domain s1.state.S.mem) /\
-      Set.equal (Map.domain s2_orig.state.S.mem) (Map.domain s2.state.S.mem) /\
-      check_if_consumes_fixed_time_outs outs args oprs ts_orig t_ins t_out /\
+      let s1t = state_with_taint s1 memTaint1 stackTaint1 in
+      let s2t = state_with_taint s2 memTaint2 stackTaint2 in
+      let s1' = S.instr_write_output_explicit i v1 o s1_orig s1 in
+      let s2' = S.instr_write_output_explicit i v2 o s2_orig s2 in
+      s1'.S.ms_ok /\ s2'.S.ms_ok /\
+      (t_out == Public ==> v1 == v2) /\
+      Set.equal (Map.domain s1_orig.S.ms_mem) (Map.domain s1.S.ms_mem) /\
+      Set.equal (Map.domain s2_orig.S.ms_mem) (Map.domain s2.S.ms_mem) /\
+      check_if_consumes_fixed_time_outs_explicit i o ts_orig t_ins t_out /\
       publicValuesAreSame ts_orig s1_orig s2_orig /\
-      publicValuesAreSame ts s1 s2
+      publicValuesAreSame ts s1t s2t
     ))
     (ensures (
-      let memTaint1, stackTaint1 = update_taint_outputs outs args oprs t_ins s1.memTaint s1.stackTaint s1_orig.state in
-      let s1' = {
-        state = S.instr_write_outputs outs args vs1 oprs s1_orig.state s1.state;
-        trace = s1.trace;
-        memTaint = memTaint1;
-        stackTaint = stackTaint1;
-      } in
-      let memTaint2, stackTaint2 = update_taint_outputs outs args oprs t_ins s2.memTaint s2.stackTaint s2_orig.state in
-      let s2' = {
-        state = S.instr_write_outputs outs args vs2 oprs s2_orig.state s2.state;
-        trace = s2.trace;
-        memTaint = memTaint2;
-        stackTaint = stackTaint2;
-      } in
+      let (memTaint1', stackTaint1') =
+        update_taint_operand_explicit i o t_ins memTaint1 stackTaint1 s1_orig in
+      let s1' = S.instr_write_output_explicit i v1 o s1_orig s1 in
+      let (memTaint2', stackTaint2') =
+        update_taint_operand_explicit i o t_ins memTaint2 stackTaint2 s2_orig in
+      let s2' = S.instr_write_output_explicit i v2 o s2_orig s2 in
+      let ts' = instr_set_taint_explicit i o ts t_out in
+      let s1t' = state_with_taint s1' memTaint1' stackTaint1' in
+      let s2t' = state_with_taint s2' memTaint2' stackTaint2' in
+      Set.equal (Map.domain s1_orig.S.ms_mem) (Map.domain s1'.S.ms_mem) /\
+      Set.equal (Map.domain s2_orig.S.ms_mem) (Map.domain s2'.S.ms_mem) /\
+      publicValuesAreSame ts' s1t' s2t'
+    ))
+  =
+  lemma_preserve_valid64 s1_orig.S.ms_mem s1.S.ms_mem;
+  lemma_preserve_valid64 s2_orig.S.ms_mem s2.S.ms_mem;
+  lemma_preserve_valid128 s1_orig.S.ms_mem s1.S.ms_mem;
+  lemma_preserve_valid128 s2_orig.S.ms_mem s2.S.ms_mem;
+  let o =
+    match i with
+    | IOp64 -> (match coerce o with OMem _ | OStack _ | _ -> o)
+    | IOpXmm -> (match coerce o with Mov128Mem _ | Mov128Stack _ | _ -> o)
+    in
+  FStar.Pervasives.reveal_opaque (`%S.valid_addr128) S.valid_addr128;
+  ()
+
+let lemma_instr_set_taints_implicit
+    (i:instr_operand_implicit) (v1 v2:instr_val_t (IOpIm i))
+    (ts_orig ts:analysis_taints) (t_ins t_out:taint)
+    (s1_orig s1 s2_orig s2:S.machine_state)
+    (memTaint1 stackTaint1 memTaint2 stackTaint2:memTaint_t)
+  : Lemma
+    (requires (
+      let s1t = state_with_taint s1 memTaint1 stackTaint1 in
+      let s2t = state_with_taint s2 memTaint2 stackTaint2 in
+      let s1' = S.instr_write_output_implicit i v1 s1_orig s1 in
+      let s2' = S.instr_write_output_implicit i v2 s2_orig s2 in
+      s1'.S.ms_ok /\ s2'.S.ms_ok /\
+      (t_out == Public ==> v1 == v2) /\
+      Set.equal (Map.domain s1_orig.S.ms_mem) (Map.domain s1.S.ms_mem) /\
+      Set.equal (Map.domain s2_orig.S.ms_mem) (Map.domain s2.S.ms_mem) /\
+      check_if_consumes_fixed_time_outs_implicit i ts_orig t_ins t_out /\
+      publicValuesAreSame ts_orig s1_orig s2_orig /\
+      publicValuesAreSame ts s1t s2t
+    ))
+    (ensures (
+      let (memTaint1', stackTaint1') =
+        update_taint_operand_implicit i t_ins memTaint1 stackTaint1 s1_orig in
+      let s1' = S.instr_write_output_implicit i v1 s1_orig s1 in
+      let (memTaint2', stackTaint2') =
+        update_taint_operand_implicit i t_ins memTaint2 stackTaint2 s2_orig in
+      let s2' = S.instr_write_output_implicit i v2 s2_orig s2 in
+      let ts' = instr_set_taint_implicit i ts t_out in
+      let s1t' = state_with_taint s1' memTaint1' stackTaint1' in
+      let s2t' = state_with_taint s2' memTaint2' stackTaint2' in
+      Set.equal (Map.domain s1_orig.S.ms_mem) (Map.domain s1'.S.ms_mem) /\
+      Set.equal (Map.domain s2_orig.S.ms_mem) (Map.domain s2'.S.ms_mem) /\
+      publicValuesAreSame ts' s1t' s2t'
+    ))
+  =
+  lemma_preserve_valid64 s1_orig.S.ms_mem s1.S.ms_mem;
+  lemma_preserve_valid64 s2_orig.S.ms_mem s2.S.ms_mem;
+  lemma_preserve_valid128 s1_orig.S.ms_mem s1.S.ms_mem;
+  lemma_preserve_valid128 s2_orig.S.ms_mem s2.S.ms_mem;
+  let i =
+    match i with
+    | IOp64One (OMem _) | IOpXmmOne (Mov128Mem _) | IOp64One (OStack _) | IOpXmmOne (Mov128Stack _) | _ -> i
+    in
+  FStar.Pervasives.reveal_opaque (`%S.valid_addr128) S.valid_addr128;
+  ()
+
+#reset-options "--z3rlimit 80"
+let rec lemma_instr_set_taints
+    (outs:list instr_out) (args:list instr_operand)
+    (vs1 vs2:instr_ret_t outs) (oprs:instr_operands_t outs args)
+    (ts_orig ts:analysis_taints) (t_ins t_out:taint)
+    (s1_orig s1 s2_orig s2:S.machine_state)
+    (memTaint1 stackTaint1 memTaint2 stackTaint2:memTaint_t)
+  : Lemma
+    (requires (
+      let s1_state' = S.instr_write_outputs outs args vs1 oprs s1_orig s1 in
+      let s2_state' = S.instr_write_outputs outs args vs2 oprs s2_orig s2 in
+      let s1t = state_with_taint s1 memTaint1 stackTaint1 in
+      let s2t = state_with_taint s2 memTaint2 stackTaint2 in
+      s1_state'.S.ms_ok /\ s2_state'.S.ms_ok /\
+      (t_out == Public ==> vs1 == vs2) /\
+      Set.equal (Map.domain s1_orig.S.ms_mem) (Map.domain s1.S.ms_mem) /\
+      Set.equal (Map.domain s2_orig.S.ms_mem) (Map.domain s2.S.ms_mem) /\
+      check_if_consumes_fixed_time_outs outs args oprs ts_orig t_ins t_out /\
+      publicValuesAreSame ts_orig s1_orig s2_orig /\
+      publicValuesAreSame ts s1t s2t
+    ))
+    (ensures (
+      let (memTaint1', stackTaint1') =
+        update_taint_outputs outs args oprs t_ins memTaint1 stackTaint1 s1_orig in
+      let s1' = state_with_taint (S.instr_write_outputs outs args vs1 oprs s1_orig s1)
+        memTaint1' stackTaint1' in
+      let (memTaint2', stackTaint2') =
+        update_taint_outputs outs args oprs t_ins memTaint2 stackTaint2 s2_orig in
+      let s2' = state_with_taint (S.instr_write_outputs outs args vs2 oprs s2_orig s2)
+        memTaint2' stackTaint2' in
       let ts' = instr_set_taints outs args oprs ts t_out in
       publicValuesAreSame ts' s1' s2'
     ))
@@ -367,158 +526,53 @@ let rec lemma_instr_set_taints_secret
           | IOp64 -> (match coerce o with OMem _ | OStack _ | _ -> o)
           | IOpXmm -> (match coerce o with Mov128Mem _ | Mov128Stack _ | _ -> o)
           in
-        let memTaint1, stackTaint1 = update_taint_operand_explicit i o t_ins s1.memTaint s1.stackTaint s1_orig.state in
-        let s1' = {
-          state = S.instr_write_output_explicit i v1 o s1_orig.state s1.state;
-          trace = s1.trace;
-          memTaint = memTaint1;
-          stackTaint = stackTaint1;
-        } in
-        let memTaint2, stackTaint2 = update_taint_operand_explicit i o t_ins s2.memTaint s2.stackTaint s2_orig.state in
-        let s2' = {
-          state = S.instr_write_output_explicit i v2 o s2_orig.state s2.state;
-          trace = s2.trace;
-          memTaint = memTaint2;
-          stackTaint = stackTaint2;
-        } in
-        lemma_instr_write_outputs_ok outs args vs1 oprs s1_orig.state s1'.state;
-        lemma_instr_write_outputs_ok outs args vs2 oprs s2_orig.state s2'.state;
+        let (memTaint1', stackTaint1') =
+          update_taint_operand_explicit i o t_ins memTaint1 stackTaint1 s1_orig in
+        let s1' = S.instr_write_output_explicit i v1 o s1_orig s1 in
+        let (memTaint2', stackTaint2') =
+          update_taint_operand_explicit i o t_ins memTaint2 stackTaint2 s2_orig in
+        let s2' = S.instr_write_output_explicit i v2 o s2_orig s2 in
+        lemma_instr_write_outputs_ok outs args vs1 oprs s1_orig s1';
+        lemma_instr_write_outputs_ok outs args vs2 oprs s2_orig s2';
         let ts' = instr_set_taint_explicit i o ts t_out in
-        lemma_instr_set_taints_secret outs args vs1 vs2 oprs ts_orig ts' t_ins t_out s1_orig s1' s2_orig s2'
+        lemma_instr_set_taints_explicit i v1 v2 o ts_orig ts t_ins t_out s1_orig s1 s2_orig s2
+          memTaint1 stackTaint1 memTaint2 stackTaint2;
+        lemma_instr_set_taints outs args vs1 vs2 oprs ts_orig ts' t_ins t_out
+          s1_orig s1' s2_orig s2' memTaint1' stackTaint1' memTaint2' stackTaint2'
       | IOpIm i ->
         let i = match i with IOp64One (OMem _) | IOpXmmOne (Mov128Mem _) | IOp64One (OStack _) | IOpXmmOne (Mov128Stack _) | _ -> i in
-        let memTaint1, stackTaint1 = update_taint_operand_implicit i t_ins s1.memTaint s1.stackTaint s1_orig.state in
-        let s1' = {
-          state = S.instr_write_output_implicit i v1 s1_orig.state s1.state;
-          trace = s1.trace;
-          memTaint = memTaint1;
-          stackTaint = stackTaint1;
-        } in
-        let memTaint2, stackTaint2 = update_taint_operand_implicit i t_ins s2.memTaint s2.stackTaint s2_orig.state in
-        let s2' = {
-          state = S.instr_write_output_implicit i v2 s2_orig.state s2.state;
-          trace = s2.trace;
-          memTaint = memTaint2;
-          stackTaint = stackTaint2;
-        } in
-        lemma_instr_write_outputs_ok outs args vs1 (coerce oprs) s1_orig.state s1'.state;
-        lemma_instr_write_outputs_ok outs args vs2 (coerce oprs) s2_orig.state s2'.state;
+        let (memTaint1', stackTaint1') =
+          update_taint_operand_implicit i t_ins memTaint1 stackTaint1 s1_orig in
+        let s1' = S.instr_write_output_implicit i v1 s1_orig s1 in
+        let (memTaint2', stackTaint2') =
+          update_taint_operand_implicit i t_ins memTaint2 stackTaint2 s2_orig in
+        let s2' = S.instr_write_output_implicit i v2 s2_orig s2 in
+        lemma_instr_write_outputs_ok outs args vs1 (coerce oprs) s1_orig s1';
+        lemma_instr_write_outputs_ok outs args vs2 (coerce oprs) s2_orig s2';
         let ts' = instr_set_taint_implicit i ts t_out in
-        lemma_instr_set_taints_secret outs args vs1 vs2 (coerce oprs) ts_orig ts' t_ins t_out s1_orig s1' s2_orig s2'
+        lemma_instr_set_taints_implicit i v1 v2 ts_orig ts t_ins t_out s1_orig s1 s2_orig s2
+          memTaint1 stackTaint1 memTaint2 stackTaint2;
+        lemma_instr_set_taints outs args vs1 vs2 (coerce oprs) ts_orig ts' t_ins t_out
+          s1_orig s1' s2_orig s2' memTaint1' stackTaint1' memTaint2' stackTaint2'
     )
 
-#reset-options "--z3rlimit 500"
-
-let rec lemma_instr_set_taints_public
-    (outs:list instr_out) (args:list instr_operand)
-    (vs:instr_ret_t outs) (oprs:instr_operands_t outs args) (ts_orig ts:taintState) (t_ins t_out:taint)
-    (s1_orig s1 s2_orig s2:traceState)
-  : Lemma
-    (requires (
-      let s1_state' = S.instr_write_outputs outs args vs oprs s1_orig.state s1.state in
-      let s2_state' = S.instr_write_outputs outs args vs oprs s2_orig.state s2.state in
-      s1_state'.S.ok /\ s2_state'.S.ok /\
-      t_out == Public /\ // REVIEW: not actually needed
-      Set.equal (Map.domain s1_orig.state.S.mem) (Map.domain s1.state.S.mem) /\
-      Set.equal (Map.domain s2_orig.state.S.mem) (Map.domain s2.state.S.mem) /\
-      check_if_consumes_fixed_time_outs outs args oprs ts_orig t_ins t_out /\
-      publicValuesAreSame ts_orig s1_orig s2_orig /\
-      publicValuesAreSame ts s1 s2
-    ))
-    (ensures (
-      let memTaint1, stackTaint1 = update_taint_outputs outs args oprs t_ins s1.memTaint s1.stackTaint s1_orig.state in
-      let s1' = {
-        state = S.instr_write_outputs outs args vs oprs s1_orig.state s1.state;
-        trace = s1.trace;
-        memTaint = memTaint1;
-        stackTaint = stackTaint1;
-      } in
-      let memTaint2, stackTaint2 = update_taint_outputs outs args oprs t_ins s2.memTaint s2.stackTaint s2_orig.state in
-      let s2' = {
-        state = S.instr_write_outputs outs args vs oprs s2_orig.state s2.state;
-        trace = s2.trace;
-        memTaint = memTaint2;
-        stackTaint = stackTaint2;
-      } in
-      let ts' = instr_set_taints outs args oprs ts t_out in
-      publicValuesAreSame ts' s1' s2'
-    ))
-  =
-  match outs with
-  | [] -> ()
-  | (_, i)::outs ->
-    (
-      let ((v:instr_val_t i), (vs:instr_ret_t outs)) =
-        match outs with
-        | [] -> (vs, ())
-        | _::_ -> let vs = coerce vs in (fst vs, snd vs)
-        in
-      match i with
-      | IOpEx i ->
-        let (o, oprs):instr_operand_t i & instr_operands_t outs args = coerce oprs in
-        let o =
-          match i with
-          | IOp64 -> (match coerce o with OMem _ | OStack _ | _ -> o)
-          | IOpXmm -> (match coerce o with Mov128Mem _ | Mov128Stack _ | _ -> o)
-          in
-        let memTaint1, stackTaint1 = update_taint_operand_explicit i o t_ins s1.memTaint s1.stackTaint s1_orig.state in
-        let s1' = {
-          state = S.instr_write_output_explicit i v o s1_orig.state s1.state;
-          trace = s1.trace;
-          memTaint = memTaint1;
-          stackTaint = stackTaint1;
-        } in
-        let memTaint2, stackTaint2 = update_taint_operand_explicit i o t_ins s2.memTaint s2.stackTaint s2_orig.state in
-        let s2' = {
-          state = S.instr_write_output_explicit i v o s2_orig.state s2.state;
-          trace = s2.trace;
-          memTaint = memTaint2;
-          stackTaint = stackTaint2;
-        } in
-        lemma_instr_write_outputs_ok outs args vs oprs s1_orig.state s1'.state;
-        lemma_instr_write_outputs_ok outs args vs oprs s2_orig.state s2'.state;
-        let ts' = instr_set_taint_explicit i o ts t_out in
-        lemma_instr_set_taints_public outs args vs oprs ts_orig ts' t_ins t_out s1_orig s1' s2_orig s2'
-      | IOpIm i ->
-        let i = match i with IOp64One (OMem _) | IOpXmmOne (Mov128Mem _) | IOp64One (OStack _) | IOpXmmOne (Mov128Stack _) | _ -> i in
-        let memTaint1, stackTaint1 = update_taint_operand_implicit i t_ins s1.memTaint s1.stackTaint s1_orig.state in
-        let s1' = {
-          state = S.instr_write_output_implicit i v s1_orig.state s1.state;
-          trace = s1.trace;
-          memTaint = memTaint1;
-          stackTaint = stackTaint1;
-        } in
-        let memTaint2, stackTaint2 = update_taint_operand_implicit i t_ins s2.memTaint s2.stackTaint s2_orig.state in
-        let s2' = {
-          state = S.instr_write_output_implicit i v s2_orig.state s2.state;
-          trace = s2.trace;
-          memTaint = memTaint2;
-          stackTaint = stackTaint2;
-        } in
-        lemma_instr_write_outputs_ok outs args vs (coerce oprs) s1_orig.state s1'.state;
-        lemma_instr_write_outputs_ok outs args vs (coerce oprs) s2_orig.state s2'.state;
-        let ts' = instr_set_taint_implicit i ts t_out in
-        lemma_instr_set_taints_public outs args vs (coerce oprs) ts_orig ts' t_ins t_out s1_orig s1' s2_orig s2'
-    )
-
-
-let check_if_instr_consumes_fixed_time (ins:tainted_ins) (ts:taintState) : Pure (bool & taintState)
+let check_if_instr_consumes_fixed_time (ins:tainted_ins) (ts:analysis_taints) : Pure (bool & analysis_taints)
   (requires BC.Instr? ins.i)
   (ensures ins_consumes_fixed_time ins ts)
   =
   let BC.Instr (InstrTypeRecord #outs #args #havoc_flags iins) oprs _ = ins.i in
   let t = inouts_taint outs args oprs ts ins.t in
   let b = check_if_consumes_fixed_time_outs outs args oprs ts ins.t t in
-  let TaintState rs flags cf ovf xmms = ts in
+  let AnalysisTaints rs flags cf ovf xmms = ts in
   let flags = match havoc_flags with | HavocFlags -> Secret | PreserveFlags -> flags in
   let cf = match havoc_flags with | HavocFlags -> Secret | PreserveFlags -> cf in
   let ovf = match havoc_flags with | HavocFlags -> Secret | PreserveFlags -> ovf in
-  let ts = TaintState rs flags cf ovf xmms in
+  let ts = AnalysisTaints rs flags cf ovf xmms in
   (b, instr_set_taints outs args oprs ts t)
 
 let coerce_to_normal (#a:Type0) (x:a) : y:(normal a){x == y} = x
 
-let check_if_xor_consumes_fixed_time (ins:tainted_ins) (ts:taintState) : Pure (bool & taintState)
+let check_if_xor_consumes_fixed_time (ins:tainted_ins) (ts:analysis_taints) : Pure (bool & analysis_taints)
   (requires BC.Instr? ins.i /\ S.AnnotateXor64? (BC.Instr?.annotation ins.i))
   (ensures ins_consumes_fixed_time ins ts)
   =
@@ -529,25 +583,25 @@ let check_if_xor_consumes_fixed_time (ins:tainted_ins) (ts:taintState) : Pure (b
   if o1 = o2 then
     let t = Public in
     let b = check_if_consumes_fixed_time_outs outs args oprs ts ins.t t in
-    let TaintState rs _ _ _ xmms = ts in
-    let ts = TaintState rs Secret Public Public xmms in
+    let AnalysisTaints rs _ _ _ xmms = ts in
+    let ts = AnalysisTaints rs Secret Public Public xmms in
     (b, instr_set_taints outs args oprs ts t)
   else
     check_if_instr_consumes_fixed_time ins ts
 
-let check_if_alloc_consumes_fixed_time (ins:tainted_ins) (ts:taintState) : Pure (bool & taintState)
+let check_if_alloc_consumes_fixed_time (ins:tainted_ins) (ts:analysis_taints) : Pure (bool & analysis_taints)
   (requires BC.Alloc? ins.i)
   (ensures ins_consumes_fixed_time ins ts)
   = true, ts
 
-let check_if_dealloc_consumes_fixed_time (ins:tainted_ins) (ts:taintState) : Pure (bool & taintState)
+let check_if_dealloc_consumes_fixed_time (ins:tainted_ins) (ts:analysis_taints) : Pure (bool & analysis_taints)
   (requires BC.Dealloc? ins.i)
   (ensures ins_consumes_fixed_time ins ts)
   = true, ts
   
 #reset-options "--initial_ifuel 2 --max_ifuel 2 --initial_fuel 4 --max_fuel 4 --z3rlimit 80"
 
-let check_if_push_consumes_fixed_time (ins:tainted_ins) (ts:taintState) : Pure (bool & taintState)
+let check_if_push_consumes_fixed_time (ins:tainted_ins) (ts:analysis_taints) : Pure (bool & analysis_taints)
   (requires BC.Push? ins.i)
   (ensures ins_consumes_fixed_time ins ts)
   = 
@@ -556,7 +610,7 @@ let check_if_push_consumes_fixed_time (ins:tainted_ins) (ts:taintState) : Pure (
   let t_out = operand_taint src ts t_ins in
   Public? (ts.regTaint rRsp) && operand_does_not_use_secrets src ts && (t_out = Public || t_ins = Secret), ts
 
-let check_if_pop_consumes_fixed_time (ins:tainted_ins) (ts:taintState) : Pure (bool & taintState)
+let check_if_pop_consumes_fixed_time (ins:tainted_ins) (ts:analysis_taints) : Pure (bool & analysis_taints)
   (requires BC.Pop? ins.i)
   (ensures ins_consumes_fixed_time ins ts)
   = 
@@ -573,7 +627,7 @@ let check_if_ins_consumes_fixed_time ins ts =
   | BC.Dealloc _ -> check_if_dealloc_consumes_fixed_time ins ts
 
 #reset-options "--initial_ifuel 1 --max_ifuel 1 --initial_fuel 1 --max_fuel 1 --z3rlimit 100"
-let lemma_instr_leakage_free (ts:taintState) (ins:tainted_ins) : Lemma
+let lemma_instr_leakage_free (ts:analysis_taints) (ins:tainted_ins) : Lemma
   (requires BC.Instr? ins.i)
   (ensures (
     let (b, ts') = check_if_instr_consumes_fixed_time ins ts in
@@ -584,7 +638,7 @@ let lemma_instr_leakage_free (ts:taintState) (ins:tainted_ins) : Lemma
   if b then
   (
     let code = Ins ins in
-    let lem (s1 s2:traceState) (fuel:nat) : Lemma
+    let lem (s1 s2:S.machine_state) (fuel:nat) : Lemma
       (requires is_explicit_leakage_free_lhs code fuel ts ts' s1 s2)
       (ensures is_explicit_leakage_free_rhs code fuel ts ts' s1 s2)
       [SMTPat (is_explicit_leakage_free_rhs code fuel ts ts' s1 s2)]
@@ -592,34 +646,38 @@ let lemma_instr_leakage_free (ts:taintState) (ins:tainted_ins) : Lemma
       let BC.Instr (InstrTypeRecord #outs #args #havoc_flags i) oprs _ = ins.i in
       let t_ins = ins.t in
       let t_out = inouts_taint outs args oprs ts ins.t in
-      let Some vs1 = S.instr_apply_eval outs args (instr_eval i) oprs s1.state in
-      let Some vs2 = S.instr_apply_eval outs args (instr_eval i) oprs s2.state in
+      let s1 = {s1 with S.ms_trace = []} in
+      let s2 = {s2 with S.ms_trace = []} in
+      let Some vs1 = S.instr_apply_eval outs args (instr_eval i) oprs s1 in
+      let Some vs2 = S.instr_apply_eval outs args (instr_eval i) oprs s2 in
       let s1' =
         match havoc_flags with
-        | HavocFlags -> {s1 with state = {s1.state with S.flags = S.havoc s1.state ins.i}}
+        | HavocFlags -> {s1 with S.ms_flags = S.havoc_state_ins s1 ins.i}
         | PreserveFlags -> s1
         in
       let s2' =
         match havoc_flags with
-        | HavocFlags -> {s2 with state = {s2.state with S.flags = S.havoc s2.state ins.i}}
+        | HavocFlags -> {s2 with S.ms_flags = S.havoc_state_ins s2 ins.i}
         | PreserveFlags -> s2
         in
-      let TaintState rs flags cf ovf xmms = ts in
+      let AnalysisTaints rs flags cf ovf xmms = ts in
       let flags = match havoc_flags with | HavocFlags -> Secret | PreserveFlags -> flags in
       let cf = match havoc_flags with | HavocFlags -> Secret | PreserveFlags -> cf in
       let ovf = match havoc_flags with | HavocFlags -> Secret | PreserveFlags -> ovf in
-      let ts_havoc = TaintState rs flags cf ovf xmms in
+      let ts_havoc = AnalysisTaints rs flags cf ovf xmms in
 
       if t_out = Secret then
       (
-        lemma_instr_set_taints_secret outs args vs1 vs2 oprs ts ts_havoc t_ins t_out s1 s1' s2 s2';
+        lemma_instr_set_taints outs args vs1 vs2 oprs ts ts_havoc t_ins t_out s1 s1' s2 s2'
+          s1.S.ms_memTaint s1.S.ms_stackTaint s2.S.ms_memTaint s2.S.ms_stackTaint;
         ()
       )
       else
       (
         let vs = vs1 in
         lemma_inouts_taint outs outs args (instr_eval i) oprs ts t_ins s1 s2;
-        lemma_instr_set_taints_public outs args vs oprs ts ts_havoc t_ins t_out s1 s1' s2 s2';
+        lemma_instr_set_taints outs args vs vs oprs ts ts_havoc t_ins t_out s1 s1' s2 s2'
+          s1.S.ms_memTaint s1.S.ms_stackTaint s2.S.ms_memTaint s2.S.ms_stackTaint;
         ()
       )
       in
@@ -627,7 +685,7 @@ let lemma_instr_leakage_free (ts:taintState) (ins:tainted_ins) : Lemma
     ()
   )
 
-let lemma_dealloc_leakage_free (ts:taintState) (ins:tainted_ins) : Lemma
+let lemma_dealloc_leakage_free (ts:analysis_taints) (ins:tainted_ins) : Lemma
   (requires BC.Dealloc? ins.i)
   (ensures (
     let (b, ts') = check_if_dealloc_consumes_fixed_time ins ts in
@@ -638,7 +696,7 @@ let lemma_dealloc_leakage_free (ts:taintState) (ins:tainted_ins) : Lemma
   if b then
   (
     let code = Ins ins in
-    let lem (s1 s2:traceState) (fuel:nat) : Lemma
+    let lem (s1 s2:S.machine_state) (fuel:nat) : Lemma
       (requires is_explicit_leakage_free_lhs code fuel ts ts' s1 s2)
       (ensures is_explicit_leakage_free_rhs code fuel ts ts' s1 s2)
       [SMTPat (is_explicit_leakage_free_rhs code fuel ts ts' s1 s2)]
@@ -647,13 +705,13 @@ let lemma_dealloc_leakage_free (ts:taintState) (ins:tainted_ins) : Lemma
       let t_ins = ins.t in
       let s1' = Some?.v (taint_eval_code code fuel s1) in
       let s2' = Some?.v (taint_eval_code code fuel s2) in
-      let S.Vale_stack _ stack1 = s1.state.S.stack in
-      let S.Vale_stack _ stack2 = s2.state.S.stack in
-      let S.Vale_stack _ stack1' = s1'.state.S.stack in
-      let S.Vale_stack _ stack2' = s2'.state.S.stack in
+      let S.Vale_stack _ stack1 = s1.S.ms_stack in
+      let S.Vale_stack _ stack2 = s2.S.ms_stack in
+      let S.Vale_stack _ stack1' = s1'.S.ms_stack in
+      let S.Vale_stack _ stack2' = s2'.S.ms_stack in
       let aux (x:int) : Lemma
-        (requires publicStackValueIsSame stack1 stack2 s1.stackTaint s2.stackTaint x)
-        (ensures publicStackValueIsSame stack1' stack2' s1'.stackTaint s2'.stackTaint x)
+        (requires publicStackValueIsSame stack1 stack2 s1.S.ms_stackTaint s2.S.ms_stackTaint x)
+        (ensures publicStackValueIsSame stack1' stack2' s1'.S.ms_stackTaint s2'.S.ms_stackTaint x)
         = 
         Classical.forall_intro (fun s -> Vale.Set.lemma_sel_restrict s stack1 x);
         Classical.forall_intro (fun s -> Vale.Set.lemma_sel_restrict s stack2 x)
@@ -662,7 +720,7 @@ let lemma_dealloc_leakage_free (ts:taintState) (ins:tainted_ins) : Lemma
     ()
   )
 
-let lemma_push_leakage_free (ts:taintState) (ins:tainted_ins) : Lemma
+let lemma_push_leakage_free (ts:analysis_taints) (ins:tainted_ins) : Lemma
   (requires BC.Push? ins.i)
   (ensures (
     let (b, ts') = check_if_push_consumes_fixed_time ins ts in
@@ -673,7 +731,7 @@ let lemma_push_leakage_free (ts:taintState) (ins:tainted_ins) : Lemma
   if b then
   (
     let code = Ins ins in
-    let lem (s1 s2:traceState) (fuel:nat) : Lemma
+    let lem (s1 s2:S.machine_state) (fuel:nat) : Lemma
       (requires is_explicit_leakage_free_lhs code fuel ts ts' s1 s2)
       (ensures is_explicit_leakage_free_rhs code fuel ts ts' s1 s2)
       [SMTPat (is_explicit_leakage_free_rhs code fuel ts ts' s1 s2)]
@@ -683,14 +741,14 @@ let lemma_push_leakage_free (ts:taintState) (ins:tainted_ins) : Lemma
       let t_out = operand_taint src ts t_ins in
       let s1' = Some?.v (taint_eval_code code fuel s1) in
       let s2' = Some?.v (taint_eval_code code fuel s2) in
-      let S.Vale_stack _ stack1 = s1.state.S.stack in
-      let S.Vale_stack _ stack2 = s2.state.S.stack in
-      let S.Vale_stack _ stack1' = s1'.state.S.stack in
-      let S.Vale_stack _ stack2' = s2'.state.S.stack in
-      let ptr1 = S.eval_reg rRsp s1.state - 8 in
-      let ptr2 = S.eval_reg rRsp s2.state - 8 in
-      let v1 = S.eval_operand src s1.state in
-      let v2 = S.eval_operand src s2.state in
+      let S.Vale_stack _ stack1 = s1.S.ms_stack in
+      let S.Vale_stack _ stack2 = s2.S.ms_stack in
+      let S.Vale_stack _ stack1' = s1'.S.ms_stack in
+      let S.Vale_stack _ stack2' = s2'.S.ms_stack in
+      let ptr1 = S.eval_reg rRsp s1 - 8 in
+      let ptr2 = S.eval_reg rRsp s2 - 8 in
+      let v1 = S.eval_operand src s1 in
+      let v2 = S.eval_operand src s2 in
       assert (ptr1 == ptr2);
       if t_out = Secret then ()
       else (
@@ -705,7 +763,7 @@ let lemma_push_leakage_free (ts:taintState) (ins:tainted_ins) : Lemma
     ()
   )
 
-let lemma_pop_leakage_free (ts:taintState) (ins:tainted_ins) : Lemma
+let lemma_pop_leakage_free (ts:analysis_taints) (ins:tainted_ins) : Lemma
   (requires BC.Pop? ins.i)
   (ensures (
     let (b, ts') = check_if_pop_consumes_fixed_time ins ts in
@@ -716,7 +774,7 @@ let lemma_pop_leakage_free (ts:taintState) (ins:tainted_ins) : Lemma
   if b then
   (
     let code = Ins ins in
-    let lem (s1 s2:traceState) (fuel:nat) : Lemma
+    let lem (s1 s2:S.machine_state) (fuel:nat) : Lemma
       (requires is_explicit_leakage_free_lhs code fuel ts ts' s1 s2)
       (ensures is_explicit_leakage_free_rhs code fuel ts ts' s1 s2)
       [SMTPat (is_explicit_leakage_free_rhs code fuel ts ts' s1 s2)]
@@ -726,8 +784,8 @@ let lemma_pop_leakage_free (ts:taintState) (ins:tainted_ins) : Lemma
       let s1' = Some?.v (taint_eval_code code fuel s1) in
       let s2' = Some?.v (taint_eval_code code fuel s2) in
       let stack_op = OStack (MReg rRsp 0) in
-      let v1 = S.eval_operand stack_op s1.state in
-      let v2 = S.eval_operand stack_op s2.state in
+      let v1 = S.eval_operand stack_op s1 in
+      let v2 = S.eval_operand stack_op s2 in
       if ins.t = Secret then (
         match dst with
         | OReg _ -> ()
@@ -749,7 +807,7 @@ let lemma_pop_leakage_free (ts:taintState) (ins:tainted_ins) : Lemma
 
 
 #reset-options "--initial_ifuel 1 --max_ifuel 1 --initial_fuel 4 --max_fuel 4 --z3rlimit 40"
-let lemma_xor_leakage_free (ts:taintState) (ins:tainted_ins) : Lemma
+let lemma_xor_leakage_free (ts:analysis_taints) (ins:tainted_ins) : Lemma
   (requires BC.Instr? ins.i /\ S.AnnotateXor64? (BC.Instr?.annotation ins.i))
   (ensures (
     let (b, ts') = check_if_xor_consumes_fixed_time ins ts in
