vale/specs/hardware/X64.Taint_Semantics_s.fst
@@ -14,41 +14,34 @@ type map (key:eqtype) (value:Type) = Map.t key value
 unfold let op_String_Access (#a:eqtype) (#b:Type) (x:Map.t a b) (y:a) : Tot b = Map.sel x y
 unfold let op_String_Assignment = Map.upd
 
-noeq type traceState = {
-  state: state;
-  trace: list observation;
-  memTaint: memTaint_t;
-  stackTaint: memTaint_t;
-}
-
 noeq
 type tainted_ins =
   | TaintedIns: i:ins -> t:taint -> tainted_ins
 
-let operand_obs (s:traceState) (o:operand) : list observation =
+let operand_obs (s:machine_state) (o:operand) : list observation =
   match o with
     | OConst _ | OReg _ -> []
     | OMem m | OStack m ->
       match m with
       | MConst _ -> []
-      | MReg reg _ -> [MemAccess (eval_reg reg s.state)]
-      | MIndex base _ index _ -> [MemAccessOffset (eval_reg base s.state) (eval_reg index s.state)]
+      | MReg reg _ -> [MemAccess (eval_reg reg s)]
+      | MIndex base _ index _ -> [MemAccessOffset (eval_reg base s) (eval_reg index s)]
 
 [@instr_attr]
-let operand_obs128 (s:traceState) (op:mov128_op) : list observation =
+let operand_obs128 (s:machine_state) (op:mov128_op) : list observation =
   match op with
   | Mov128Xmm _ -> []
   | Mov128Stack m | Mov128Mem m -> 
       match m with
       | MConst _ -> []
-      | MReg reg _ -> [MemAccess (eval_reg reg s.state)]
-      | MIndex base _ index _ -> [MemAccessOffset (eval_reg base s.state) (eval_reg index s.state)]
+      | MReg reg _ -> [MemAccess (eval_reg reg s)]
+      | MIndex base _ index _ -> [MemAccessOffset (eval_reg base s) (eval_reg index s)]
 
 [@instr_attr]
 let obs_operand_explicit
   (i:instr_operand_explicit)
   (o:instr_operand_t i)
-  (s:traceState) : list observation =
+  (s:machine_state) : list observation =
   match i with
   | IOp64 -> operand_obs s o
   | IOpXmm -> operand_obs128 s o
@@ -56,7 +49,7 @@ let obs_operand_explicit
 [@instr_attr]
 let obs_operand_implicit
   (i:instr_operand_implicit)
-  (s:traceState) : list observation =
+  (s:machine_state) : list observation =
   match i with
   | IOp64One o -> operand_obs s o
   | IOpXmmOne o -> operand_obs128 s o
@@ -66,7 +59,7 @@ let obs_operand_implicit
 let rec obs_args
   (args:list instr_operand)
   (oprs:instr_operands_t_args args)
-  (s:traceState) : list observation =
+  (s:machine_state) : list observation =
   match args with
   | [] -> []
   | i::args ->
@@ -82,7 +75,7 @@ let rec obs_inouts
   (inouts:list instr_out) 
   (args:list instr_operand)
   (oprs:instr_operands_t inouts args)
-  (s:traceState) : list observation =
+  (s:machine_state) : list observation =
   match inouts with
   | [] -> obs_args args oprs s
   | (Out, i)::inouts -> 
@@ -100,7 +93,7 @@ let rec obs_inouts
     in v @ obs_inouts inouts args oprs s
 
 [@instr_attr]
-let ins_obs (ins:ins) (s:traceState) : list observation =
+let ins_obs (ins:ins) (s:machine_state) : list observation =
   match ins with
   | BC.Instr (InstrTypeRecord #outs #args _) oprs _ -> obs_inouts outs args oprs s
   | BC.Push src -> operand_obs s src
@@ -128,17 +121,17 @@ let rec update_n (addr:int) (n:nat) (memTaint:memTaint_t) (t:taint)
 
 (* Checks if the taint of an operand matches the ins annotation *)
 [@instr_attr]
-let taint_match (o:operand) (t:taint) (memTaint:memTaint_t) (stackTaint:memTaint_t) (s:state) : bool =
+let taint_match (o:operand) (t:taint) (memTaint:memTaint_t) (ms_stackTaint:memTaint_t) (s:machine_state) : bool =
   match o with
     | OConst _ | OReg _ -> true
     | OMem m -> match_n (eval_maddr m s) 8 memTaint t
-    | OStack m -> match_n (eval_maddr m s) 8 stackTaint t 
+    | OStack m -> match_n (eval_maddr m s) 8 ms_stackTaint t 
 
 [@instr_attr]
-let taint_match128 (op:mov128_op) (t:taint) (memTaint:memTaint_t) (stackTaint:memTaint_t) (s:state) : bool =
+let taint_match128 (op:mov128_op) (t:taint) (memTaint:memTaint_t) (ms_stackTaint:memTaint_t) (s:machine_state) : bool =
   match op with
   | Mov128Xmm _ -> true
-  | Mov128Stack addr -> match_n (eval_maddr addr s) 16 stackTaint t
+  | Mov128Stack addr -> match_n (eval_maddr addr s) 16 ms_stackTaint t
   | Mov128Mem addr -> match_n (eval_maddr addr s) 16 memTaint t
 
 [@instr_attr]
@@ -147,22 +140,22 @@ let taint_match_operand_explicit
   (o:instr_operand_t i)
   (t:taint)
   (memTaint:memTaint_t)
-  (stackTaint:memTaint_t)
-  (s:state) : bool =
+  (ms_stackTaint:memTaint_t)
+  (s:machine_state) : bool =
   match i with
-  | IOp64 -> taint_match o t memTaint stackTaint s
-  | IOpXmm -> taint_match128 o t memTaint stackTaint s
+  | IOp64 -> taint_match o t memTaint ms_stackTaint s
+  | IOpXmm -> taint_match128 o t memTaint ms_stackTaint s
 
 [@instr_attr]
 let taint_match_operand_implicit
   (i:instr_operand_implicit)
   (t:taint)
   (memTaint:memTaint_t)
-  (stackTaint:memTaint_t)
-  (s:state) : bool =
+  (ms_stackTaint:memTaint_t)
+  (s:machine_state) : bool =
   match i with
-  | IOp64One o -> taint_match o t memTaint stackTaint s
-  | IOpXmmOne o -> taint_match128 o t memTaint stackTaint s
+  | IOp64One o -> taint_match o t memTaint ms_stackTaint s
+  | IOpXmmOne o -> taint_match128 o t memTaint ms_stackTaint s
   // We only check for memory operands in trusted semantics. Taint tracking for other operands will occur in the verified taint analysis
   | IOpFlagsCf -> true
   | IOpFlagsOf -> true
@@ -173,17 +166,17 @@ let rec taint_match_args
   (oprs:instr_operands_t_args args)
   (t:taint)
   (memTaint:memTaint_t)
-  (stackTaint:memTaint_t)
-  (s:state) : bool =
+  (ms_stackTaint:memTaint_t)
+  (s:machine_state) : bool =
   match args with
   | [] -> true
   | i::args ->
     match i with
     | IOpEx i -> let oprs = coerce oprs in
-                taint_match_operand_explicit i (fst oprs) t memTaint stackTaint s &&
-                 taint_match_args args (snd oprs) t memTaint stackTaint s
-    | IOpIm i -> taint_match_operand_implicit i t memTaint stackTaint s &&
-                 taint_match_args args (coerce oprs) t memTaint stackTaint s
+                taint_match_operand_explicit i (fst oprs) t memTaint ms_stackTaint s &&
+                 taint_match_args args (snd oprs) t memTaint ms_stackTaint s
+    | IOpIm i -> taint_match_operand_implicit i t memTaint ms_stackTaint s &&
+                 taint_match_args args (coerce oprs) t memTaint ms_stackTaint s
 
 [@instr_attr]
 let rec taint_match_inouts 
@@ -192,45 +185,45 @@ let rec taint_match_inouts
   (oprs:instr_operands_t inouts args)
   (t:taint)
   (memTaint:memTaint_t)
-  (stackTaint:memTaint_t)
-  (s:state) : bool =
+  (ms_stackTaint:memTaint_t)
+  (s:machine_state) : bool =
   match inouts with
-  | [] -> taint_match_args args oprs t memTaint stackTaint s
+  | [] -> taint_match_args args oprs t memTaint ms_stackTaint s
   | (Out, i)::inouts -> 
     let oprs =
       match i with
       | IOpEx i -> snd #(instr_operand_t i) (coerce oprs)
       | IOpIm i -> coerce oprs
-    in taint_match_inouts inouts args oprs t memTaint stackTaint s
+    in taint_match_inouts inouts args oprs t memTaint ms_stackTaint s
   | (InOut, i)::inouts -> 
     let (v, oprs) =
       match i with
       | IOpEx i -> let oprs = coerce oprs in
-              (taint_match_operand_explicit i (fst oprs) t memTaint stackTaint s), snd oprs
-      | IOpIm i -> taint_match_operand_implicit i t memTaint stackTaint s, coerce oprs
-    in v && taint_match_inouts inouts args oprs t memTaint stackTaint s
+              (taint_match_operand_explicit i (fst oprs) t memTaint ms_stackTaint s), snd oprs
+      | IOpIm i -> taint_match_operand_implicit i t memTaint ms_stackTaint s, coerce oprs
+    in v && taint_match_inouts inouts args oprs t memTaint ms_stackTaint s
 
 [@instr_attr]
-let taint_match_ins (ins:ins) (t:taint) (memTaint:memTaint_t) (stackTaint:memTaint_t) (s:state) : bool =
+let taint_match_ins (ins:ins) (t:taint) (memTaint:memTaint_t) (ms_stackTaint:memTaint_t) (s:machine_state) : bool =
   match ins with
-  | BC.Instr (InstrTypeRecord #outs #args _) oprs _ -> taint_match_inouts outs args oprs t memTaint stackTaint s
-  | BC.Push src -> taint_match src t memTaint stackTaint s
-  | BC.Pop _ -> taint_match (OStack (MReg rRsp 0)) t memTaint stackTaint s
+  | BC.Instr (InstrTypeRecord #outs #args _) oprs _ -> taint_match_inouts outs args oprs t memTaint ms_stackTaint s
+  | BC.Push src -> taint_match src t memTaint ms_stackTaint s
+  | BC.Pop _ -> taint_match (OStack (MReg rRsp 0)) t memTaint ms_stackTaint s
   | BC.Alloc _ | BC.Dealloc _ -> true
 
 [@instr_attr]
-let update_taint (memTaint:memTaint_t) (stackTaint:memTaint_t) (dst:operand) (t:taint) (s:state) : memTaint_t * memTaint_t =
+let update_taint (memTaint:memTaint_t) (ms_stackTaint:memTaint_t) (dst:operand) (t:taint) (s:machine_state) : memTaint_t * memTaint_t =
   match dst with
-    | OConst _ | OReg _ -> memTaint, stackTaint
-    | OMem m -> update_n (eval_maddr m s) 8 memTaint t, stackTaint
-    | OStack m -> memTaint, update_n (eval_maddr m s) 8 stackTaint t
+    | OConst _ | OReg _ -> memTaint, ms_stackTaint
+    | OMem m -> update_n (eval_maddr m s) 8 memTaint t, ms_stackTaint
+    | OStack m -> memTaint, update_n (eval_maddr m s) 8 ms_stackTaint t
     
 [@instr_attr]
-let update_taint128 op t (memTaint:memTaint_t) (stackTaint:memTaint_t) (s:state) : memTaint_t * memTaint_t =
+let update_taint128 op t (memTaint:memTaint_t) (ms_stackTaint:memTaint_t) (s:machine_state) : memTaint_t * memTaint_t =
   match op with
-  | Mov128Xmm _ -> memTaint, stackTaint
-  | Mov128Mem addr -> update_n (eval_maddr addr s) 16 memTaint t, stackTaint
-  | Mov128Stack addr -> memTaint, update_n (eval_maddr addr s) 16 stackTaint t
+  | Mov128Xmm _ -> memTaint, ms_stackTaint
+  | Mov128Mem addr -> update_n (eval_maddr addr s) 16 memTaint t, ms_stackTaint
+  | Mov128Stack addr -> memTaint, update_n (eval_maddr addr s) 16 ms_stackTaint t
 
 [@instr_attr]
 let update_taint_operand_explicit
@@ -238,25 +231,25 @@ let update_taint_operand_explicit
   (o:instr_operand_t i)
   (t:taint)
   (memTaint:memTaint_t)
-  (stackTaint:memTaint_t)
-  (s:state) : memTaint_t * memTaint_t =
+  (ms_stackTaint:memTaint_t)
+  (s:machine_state) : memTaint_t * memTaint_t =
   match i with
-  | IOp64 -> update_taint memTaint stackTaint o t s
-  | IOpXmm -> update_taint128 o t memTaint stackTaint s
+  | IOp64 -> update_taint memTaint ms_stackTaint o t s
+  | IOpXmm -> update_taint128 o t memTaint ms_stackTaint s
 
 [@instr_attr]
 let update_taint_operand_implicit
   (i:instr_operand_implicit)
   (t:taint)
   (memTaint:memTaint_t)
-  (stackTaint:memTaint_t)
-  (s:state) : memTaint_t * memTaint_t =
+  (ms_stackTaint:memTaint_t)
+  (s:machine_state) : memTaint_t * memTaint_t =
   match i with
-  | IOp64One o -> update_taint memTaint stackTaint o t s
-  | IOpXmmOne o -> update_taint128 o t memTaint stackTaint s
+  | IOp64One o -> update_taint memTaint ms_stackTaint o t s
+  | IOpXmmOne o -> update_taint128 o t memTaint ms_stackTaint s
   // We only check for memory operands in trusted semantics. Taint tracking for other operands will occur in the verified taint analysis
-  | IOpFlagsCf -> memTaint, stackTaint
-  | IOpFlagsOf -> memTaint, stackTaint
+  | IOpFlagsCf -> memTaint, ms_stackTaint
+  | IOpFlagsOf -> memTaint, ms_stackTaint
 
 [@instr_attr]
 let rec update_taint_outputs
@@ -265,36 +258,35 @@ let rec update_taint_outputs
   (oprs:instr_operands_t outs args)
   (t:taint)
   (memTaint:memTaint_t)
-  (stackTaint:memTaint_t)  
-  (s:state) : memTaint_t * memTaint_t =
+  (ms_stackTaint:memTaint_t)  
+  (s:machine_state) : memTaint_t * memTaint_t =
   match outs with
-  | [] -> memTaint, stackTaint
+  | [] -> memTaint, ms_stackTaint
   | (_, i)::outs -> 
-    let (memTaint, stackTaint), oprs =
+    let (memTaint, ms_stackTaint), oprs =
       match i with
       | IOpEx i -> let oprs = coerce oprs in
-          update_taint_operand_explicit i (fst oprs) t memTaint stackTaint s, snd oprs
-      | IOpIm i -> update_taint_operand_implicit i t memTaint stackTaint s, coerce oprs
+          update_taint_operand_explicit i (fst oprs) t memTaint ms_stackTaint s, snd oprs
+      | IOpIm i -> update_taint_operand_implicit i t memTaint ms_stackTaint s, coerce oprs
    in
-   update_taint_outputs outs args oprs t memTaint stackTaint s
+   update_taint_outputs outs args oprs t memTaint ms_stackTaint s
 
 [@instr_attr]
-let update_taint_ins (ins:ins) (t:taint) (memTaint:memTaint_t) (stackTaint:memTaint_t) (s:state) : memTaint_t * memTaint_t =
+let update_taint_ins (ins:ins) (t:taint) (memTaint:memTaint_t) (ms_stackTaint:memTaint_t) (s:machine_state) : memTaint_t * memTaint_t =
   match ins with
-  | BC.Instr (InstrTypeRecord #outs #args _) oprs _ -> update_taint_outputs outs args oprs t memTaint stackTaint s
-  | BC.Alloc _ | BC.Dealloc _ -> memTaint, stackTaint
-  | BC.Push _ -> update_taint memTaint stackTaint (OStack (MReg rRsp (-8))) t s
-  | BC.Pop dst -> update_taint memTaint stackTaint dst t s
+  | BC.Instr (InstrTypeRecord #outs #args _) oprs _ -> update_taint_outputs outs args oprs t memTaint ms_stackTaint s
+  | BC.Alloc _ | BC.Dealloc _ -> memTaint, ms_stackTaint
+  | BC.Push _ -> update_taint memTaint ms_stackTaint (OStack (MReg rRsp (-8))) t s
+  | BC.Pop dst -> update_taint memTaint ms_stackTaint dst t s
 
 [@instr_attr]
-let taint_eval_ins (ins:tainted_ins) (ts: traceState) : GTot traceState =
+let taint_eval_ins (ins:tainted_ins) (ts: machine_state) : GTot machine_state =
   let t = ins.t in
   let i = ins.i in
-  let s = run (check (taint_match_ins i t ts.memTaint ts.stackTaint)) ts.state in
-  let memTaint, stackTaint = update_taint_ins i t ts.memTaint ts.stackTaint s in
-
+  let s = run (check (taint_match_ins i t ts.ms_memTaint ts.ms_stackTaint)) ts in
+  let (memTaint, ms_stackTaint) = update_taint_ins i t ts.ms_memTaint ts.ms_stackTaint s in
   let s = run (eval_ins i) s in
-  {state = s; trace = ts.trace; memTaint = memTaint; stackTaint = stackTaint}
+  {s with ms_memTaint = memTaint; ms_stackTaint = ms_stackTaint}
 
 type tainted_ocmp : eqtype = | TaintedOCmp: o:ocmp -> ot:taint -> tainted_ocmp
 
@@ -304,38 +296,41 @@ let get_fst_ocmp (o:ocmp) = match o with
 let get_snd_ocmp (o:ocmp) = match o with
   | BC.OEq _ o2 | BC.ONe _ o2 | BC.OLe _ o2 | BC.OGe _ o2 | BC.OLt _ o2 | BC.OGt _ o2 -> o2
 
-let taint_eval_ocmp (ts:traceState) (c:tainted_ocmp) : GTot (traceState * bool) =
+let taint_eval_ocmp (ts:machine_state) (c:tainted_ocmp) : GTot (machine_state * bool) =
   let t = c.ot in
-  let s = run (
-    check (valid_ocmp c.o);; 
-    check (taint_match (get_fst_ocmp c.o) t ts.memTaint ts.stackTaint);;
-    check (taint_match (get_snd_ocmp c.o) t ts.memTaint ts.stackTaint))
-  ts.state in
-  {ts with state = s}, eval_ocmp s c.o
+  let s =
+    run (
+      check (valid_ocmp c.o);; 
+      check (taint_match (get_fst_ocmp c.o) t ts.ms_memTaint ts.ms_stackTaint);;
+      check (taint_match (get_snd_ocmp c.o) t ts.ms_memTaint ts.ms_stackTaint))
+    ts
+    in
+  (s, eval_ocmp s c.o)
 
 type tainted_code = precode tainted_ins tainted_ocmp
 type tainted_codes = list tainted_code
 
-val taint_eval_code: c:tainted_code -> fuel:nat -> s:traceState -> GTot (option traceState)
-(decreases %[fuel; c; 1])
-val taint_eval_codes: l:tainted_codes -> fuel:nat -> s:traceState -> GTot (option traceState)
-(decreases %[fuel; l])
-val taint_eval_while: c:tainted_code{While? c} -> fuel:nat -> s:traceState -> GTot (option traceState)
-(decreases %[fuel; c; 0])
+val taint_eval_code (c:tainted_code) (fuel:nat) (s:machine_state) : GTot (option machine_state)
+  (decreases %[fuel; c; 1])
+val taint_eval_codes (l:tainted_codes) (fuel:nat) (s:machine_state) : GTot (option machine_state)
+  (decreases %[fuel; l])
+val taint_eval_while (c:tainted_code{While? c}) (fuel:nat) (s:machine_state) : GTot (option machine_state)
+  (decreases %[fuel; c; 0])
 
 (* Adds the observations to the eval_code.
    Returns None if eval_code returns None *)
 let rec taint_eval_code c fuel s =
   match c with
     | Ins ins -> let obs = ins_obs ins.i s in
-      Some ({taint_eval_ins ins s with trace = obs @ s.trace})
+      // REVIEW: drop trace, then restore trace, to make clear that taint_eval_ins shouldn't depend on trace
+      Some ({taint_eval_ins ins ({s with ms_trace = []}) with ms_trace = obs @ s.ms_trace})
 
     | Block l -> taint_eval_codes l fuel s
 
     | IfElse ifCond ifTrue ifFalse ->
       let st, b = taint_eval_ocmp s ifCond in
       (* We add the BranchPredicate to the trace *)
-      let s' = {st with trace=BranchPredicate(b)::s.trace} in
+      let s' = {st with ms_trace = BranchPredicate(b)::s.ms_trace} in
       (* We evaluate the branch with the new trace *)
       if b then taint_eval_code ifTrue fuel s' else taint_eval_code ifFalse fuel s'
 
@@ -357,11 +352,11 @@ and taint_eval_while c fuel s0 =
   if fuel = 0 then None else
   let While cond body = c in
   let (s0, b) = taint_eval_ocmp s0 cond in
-  if not b then Some ({s0 with trace = BranchPredicate(false)::s0.trace})
+  if not b then Some ({s0 with ms_trace = BranchPredicate(false)::s0.ms_trace})
   else
-    let s0 = {s0 with trace = BranchPredicate(true)::s0.trace} in
+    let s0 = {s0 with ms_trace = BranchPredicate(true)::s0.ms_trace} in
     let s_opt = taint_eval_code body (fuel - 1) s0 in
     match s_opt with
     | None -> None
-    | Some s1 -> if not s1.state.ok then Some s1
+    | Some s1 -> if not s1.ms_ok then Some s1
       else taint_eval_while c (fuel - 1) s1
