vale/code/arch/x64/X64.Leakage_Ins.fsti
@@ -5,8 +5,8 @@ open X64.Taint_Semantics_s
 open X64.Leakage_s
 open X64.Leakage_Helpers
 
-val check_if_ins_consumes_fixed_time: (ins:tainted_ins) -> (ts:taintState) -> (res:(bool*taintState){ins_consumes_fixed_time ins ts res})
+val check_if_ins_consumes_fixed_time: (ins:tainted_ins) -> (ts:analysis_taints) -> (res:(bool*analysis_taints){ins_consumes_fixed_time ins ts res})
   
-val lemma_ins_leakage_free: (ts:taintState) -> (ins:tainted_ins) -> Lemma
+val lemma_ins_leakage_free: (ts:analysis_taints) -> (ins:tainted_ins) -> Lemma
  (let b, ts' = check_if_ins_consumes_fixed_time ins ts in
   (b2t b ==> isConstantTime (Ins ins) ts /\ isLeakageFree (Ins ins) ts ts'))
