vale/code/arch/x64/X64.Memory_Sems.fst
@@ -286,6 +286,7 @@ let in_bounds64 (h:mem) (b:buffer64) (i:nat{i < buffer_length b})
   = length_t_eq (TUInt64) b
 
 let bytes_valid ptr h =
+  FStar.Pervasives.reveal_opaque (`%S.valid_addr64) S.valid_addr64;
   let t = TUInt64 in
   let b = get_addr_ptr t ptr h in
   let i = get_addr_in_ptr t (buffer_length b) (buffer_addr b h) ptr 0 in
@@ -368,6 +369,7 @@ let in_bounds128 (h:mem) (b:buffer128) (i:nat{i < buffer_length b}) : Lemma
   length_t_eq TUInt128 b
 
 let bytes_valid128 ptr h =
+  FStar.Pervasives.reveal_opaque (`%S.valid_addr128) S.valid_addr128;
   let t = TUInt128 in
   let b = get_addr_ptr t ptr h in
   let i = get_addr_in_ptr t (buffer_length b) (buffer_addr b h) ptr 0 in
@@ -715,6 +717,8 @@ let low_lemma_store_mem128 b i v h =
   I.update_buffer_up_mem h b heap heap'
 
 let low_lemma_valid_mem128_64 b i h = 
+  FStar.Pervasives.reveal_opaque (`%S.valid_addr64) S.valid_addr64;
+  FStar.Pervasives.reveal_opaque (`%S.valid_addr128) S.valid_addr128;
   low_lemma_valid_mem128 b i h;
   let ptr = buffer_addr b h + 16 `op_Multiply` i in
   assert (buffer_addr b h + 16 `op_Multiply` i + 8 = ptr + 8)
@@ -756,6 +760,8 @@ let update_heap128_lo (ptr:int) (v:quad32) (mem:S.heap) : Lemma
   )
   (ensures S.update_heap128 ptr v mem ==
     S.update_heap32 (ptr+4) v.lo1 (S.update_heap32 ptr v.lo0 mem)) =
+  FStar.Pervasives.reveal_opaque (`%S.valid_addr128) S.valid_addr128;
+  Opaque_s.reveal_opaque S.update_heap128_def;
   let mem0 = S.update_heap32 ptr v.lo0 mem in
   let mem1 = S.update_heap32 (ptr+4) v.lo1 mem0 in  
   X64.Bytes_Semantics.frame_update_heap32 ptr v.lo0 mem;
@@ -779,8 +785,8 @@ let low_lemma_store_mem128_lo64 b i v h =
   Opaque_s.reveal_opaque S.update_heap32_def;
   Opaque_s.reveal_opaque insert_nat64
 
-
 let low_lemma_store_mem128_hi64 b i v h =
+  FStar.Pervasives.reveal_opaque (`%S.valid_addr128) S.valid_addr128;
   let ptr = buffer_addr b h + 16 `op_Multiply` i in
   let v128 = buffer_read b i h in
   let v' = insert_nat64_opaque v128 v 1 in
@@ -790,6 +796,7 @@ let low_lemma_store_mem128_hi64 b i v h =
   X64.Bytes_Semantics.update_heap32_get_heap32 ptr (get_heap h);
   X64.Bytes_Semantics.update_heap32_get_heap32 (ptr+4) (get_heap h);
   Opaque_s.reveal_opaque S.get_heap_val128_def;
+  Opaque_s.reveal_opaque S.update_heap128_def;
   Opaque_s.reveal_opaque S.update_heap64_def;
   Opaque_s.reveal_opaque S.update_heap32_def;
   Opaque_s.reveal_opaque insert_nat64  
