vale/code/arch/x64/X64.Stack_Sems.fst
@@ -13,6 +13,7 @@ let equiv_valid_src_stack64 ptr h = ()
 let equiv_load_stack64 ptr h = ()
 
 let free_stack_same_load start finish ptr h =
+  FStar.Pervasives.reveal_opaque (`%S.valid_addr64) S.valid_addr64;
   let S.Vale_stack _ mem = h in
   let S.Vale_stack _ mem' = S.free_stack' start finish h in
   Classical.forall_intro (Vale.Set.remove_between_reveal (Map.domain mem) start finish);
@@ -31,6 +32,7 @@ let equiv_valid_src_stack128 ptr h = ()
 let equiv_load_stack128 ptr h = ()
 
 let free_stack_same_load128 start finish ptr h =
+  FStar.Pervasives.reveal_opaque (`%S.valid_addr128) S.valid_addr128;
   let S.Vale_stack _ mem = h in
   let S.Vale_stack _ mem' = S.free_stack' start finish h in
   Classical.forall_intro (Vale.Set.remove_between_reveal (Map.domain mem) start finish);
